Substantial edits to thunk_subst_unthunk
This commit implements new relations that will hopefully work with the
new semantics with delayed ticks at some point.

- thunk_rel is removed. I'm not sure whether it was still needed, aside
  from carrying an integer.
- All clocks in proofs are removed.
- Induction in the Force-case /almost/ works. Everything else works.

compiler/backend/proofs/thunk_subst_unthunkProofScript.sml
@@ -37,7 +37,8 @@ Theorem exp_ind_alt[local]:
     (∀x. P x ⇒ P (Delay x)) ∧
     (∀x. P x ⇒ P (Box x)) ∧
     (∀x. P x ⇒ P (Force x)) ∧
-    (∀v. P (Value v)) ⇒
+    (∀v. P (Value v)) ∧
+    (∀x. P (MkTick x)) ⇒
       ∀v. P v
 Proof
   gen_tac
@@ -168,6 +169,7 @@ Theorem closed_simps[local,simp]:
   (∀x. closed (Delay x) ⇔ closed x)  ∧
   (∀x. closed (Box x) ⇔ closed x)  ∧
   (∀v. closed (Value v) ⇔ T)  ∧
+  (∀x. closed (MkTick x) ⇔ closed x) ∧
   (∀v. closed (Var v) ⇔ F)
 Proof
   rw [closed_def, freevars_def]
@@ -243,6 +245,14 @@ Inductive exp_ok:
   (∀v.
      v_ok v ⇒
        exp_ok (Value v)) ∧
+[exp_ok_MkTick:]
+  (∀x.
+     exp_ok x ⇒
+       exp_ok (MkTick x)) ∧
+[v_ok_DoTick:]
+  (∀v.
+     v_ok v ⇒
+       v_ok (DoTick v)) ∧
 [v_ok_Constructor:]
   (∀s vs.
      EVERY v_ok vs ⇒
@@ -291,7 +301,9 @@ Theorem exp_ok_def:
   (∀x.
      exp_ok (Force x) = exp_ok x) ∧
   (∀v.
-     exp_ok (Value v) = v_ok v)
+     exp_ok (Value v) = v_ok v) ∧
+  (∀x.
+     exp_ok (MkTick x) = exp_ok x)
 Proof
   rw [] \\ rw [Once exp_ok_cases]
 QED
@@ -309,6 +321,8 @@ Theorem v_ok_def:
      v_ok (Thunk (INL v)) = v_ok v) ∧
   (∀x.
      v_ok (Thunk (INR x)) = exp_ok x) ∧
+  (∀v.
+     v_ok (DoTick v) = v_ok v) ∧
   (∀x.
      v_ok (Atom x))
 Proof
@@ -347,6 +361,16 @@ Proof
     \\ simp [PULL_EXISTS]
     \\ first_assum (irule_at Any)
     \\ gs [EVERY_MEM, FORALL_PROD, SF SFY_ss])
+QED
+
+Theorem dest_Tick_v_ok[local]:
+  ∀v w n.
+    v_ok v ∧ dest_Tick v = (w, n) ⇒
+      v_ok w
+Proof
+  Induct \\ rw [] \\ gs [dest_Tick_def]
+  \\ pairarg_tac \\ gvs []
+  \\ gs [v_ok_def]
 QED
 
 Theorem exp_ok_eval_to:
@@ -435,33 +459,36 @@ Proof
   >- ((* Force *)
     gs [exp_ok_def, eval_to_def]
     \\ Cases_on ‘eval_to k x’ \\ gs []
-    \\ Cases_on ‘dest_anyThunk y’ \\ gs []
     \\ pairarg_tac \\ gvs []
-    \\ BasicProvers.TOP_CASE_TAC \\ gs []
+    \\ Cases_on ‘dest_anyThunk w’ \\ gs []
+    \\ pairarg_tac \\ gvs []
+    \\ drule_all_then assume_tac dest_Tick_v_ok
+    \\ BasicProvers.TOP_CASE_TAC \\ gvs []
     >- (
       rw []
-      \\ Cases_on ‘y’ \\ gvs [dest_anyThunk_def, CaseEqs ["option", "exp"],
-                              v_ok_def])
-    \\ IF_CASES_TAC \\ gs [] \\ rw []
+      \\ Cases_on ‘y’ \\ Cases_on ‘w’ \\ gvs [dest_anyThunk_def, v_ok_def,
+                                              CaseEqs ["option", "exp"]])
+    \\ IF_CASES_TAC \\ gs [arithmeticTheory.NOT_LESS_EQUAL]
+    \\ strip_tac
     \\ first_x_assum irule
-    \\ first_assum (irule_at Any)
+    \\ first_assum (irule_at Any) \\ gs []
     \\ gs [subst_funs_def]
     \\ irule exp_ok_subst
-    \\ Cases_on ‘y’ \\ gs [dest_anyThunk_def, v_ok_def]
-    \\ gvs [CaseEqs ["option", "exp"]]
-    \\ dxrule_then strip_assume_tac ALOOKUP_SOME_REVERSE_EL
-    \\ gvs [EVERY_EL]
-    \\ (rw []
-        >- (
-          first_x_assum (drule_then assume_tac)
-          \\ gs [EL_MAP, exp_ok_def])
-        \\ simp [EL_MAP, ELIM_UNCURRY]
-        \\ irule v_ok_Recclosure
-        \\ gs [EVERY_EL, MEM_MAP, MEM_EL, EXISTS_PROD]
-        \\ rw [Once EQ_SYM_EQ]
-        \\ first_assum (irule_at Any)
-        \\ rename1 ‘mm < LENGTH binds’
-        \\ Cases_on ‘EL mm binds’ \\ gs []))
+    \\ simp [MAP_MAP_o, combinTheory.o_DEF, LAMBDA_PROD, EVERY_MAP, v_ok_def]
+    \\ Cases_on ‘w’ \\ gs [dest_anyThunk_def, v_ok_def]
+    \\ gvs [CaseEqs ["option", "exp"], EVERY_MAP, EVERY_EL]
+    \\ dxrule_then strip_assume_tac ALOOKUP_SOME_REVERSE_EL \\ gs []
+    \\ rw [] \\ gs [EL_MAP, exp_ok_def, ELIM_UNCURRY, MEM_EL, PULL_EXISTS]
+    \\ first_x_assum (drule_then assume_tac) \\ gvs [exp_ok_def]
+    \\ gs [EVERY_EL, MEM_MAP, MEM_EL, EXISTS_PROD]
+    \\ rw [Once EQ_SYM_EQ]
+    \\ first_assum (irule_at Any)
+    \\ rename1 ‘mm < LENGTH binds’
+    \\ Cases_on ‘EL mm binds’ \\ gs [EL_MAP])
+  >- ((* MkTick *)
+    gs [exp_ok_def, eval_to_def]
+    \\ Cases_on ‘eval_to k x’ \\ gs []
+    \\ rw [] \\ gs [v_ok_def])
   >- ((* Prim *)
     gs [exp_ok_def, eval_to_def]
     \\ Cases_on ‘op’ \\ gs []
@@ -561,7 +588,7 @@ Inductive exp_inv:
      EVERY exp_inv xs ⇒
        exp_inv (Force (Prim (Proj s i) xs))) ∧
 [exp_inv_Prim:]
-  (∀op xs. (* TODO *)
+  (∀op xs.
      (∀nm. op ≠ Cons nm) ∧
      (∀s i. op ≠ Proj s i) ∧
      EVERY exp_inv xs ⇒
@@ -665,7 +692,7 @@ Theorem v_inv_def[simp]:
   (∀x. v_inv (Thunk (INR x)) = exp_inv x) ∧
   (∀x. v_inv (Atom x) = T)
 Proof
-  rw [] \\ rw [Once exp_inv_cases]
+  rw [] \\ rw [Once exp_inv_cases, AC CONJ_COMM CONJ_ASSOC]
 QED
 
 Theorem thunk_inv_def[simp]:
@@ -675,7 +702,8 @@ Theorem thunk_inv_def[simp]:
   (∀t. thunk_inv (Thunk t) = (∃x. t = INR x ∧ exp_inv x)) ∧
   (∀s vs. ¬thunk_inv (Constructor s vs)) ∧
   (∀s x. ¬thunk_inv (Closure s x)) ∧
-  (∀x. ¬thunk_inv (Atom x))
+  (∀x. ¬thunk_inv (Atom x)) ∧
+  (∀x. ¬thunk_inv (DoTick x))
 Proof
   rw [] \\ rw [Once exp_inv_cases, SF DNF_ss]
 QED
@@ -694,12 +722,6 @@ QED
 
  *)
 
-Definition is_thunky_def[simp]:
-  is_thunky (Thunk (INR x)) = T ∧
-  is_thunky (Recclosure f n) = EVERY (λx. ∃y. x = Delay y) (MAP SND f) ∧
-  is_thunky _ = F
-End
-
 Definition is_delay_def[simp]:
   is_delay (Delay x) = T ∧
   is_delay _ = F
@@ -708,11 +730,11 @@ End
 Inductive exp_rel:
 [exp_rel_Var:]
   (∀v.
-     exp_rel (Delay (Force (Var v))) (Var v)) ∧
+     exp_rel (Delay (Force (Var v))) (MkTick (Var v))) ∧
 [exp_rel_Value:]
-  (∀n v w.
-     thunk_rel n v w ⇒
-       exp_rel (Delay (Force (Value v))) (Value w)) ∧
+  (∀v w.
+     v_rel v w ⇒
+       exp_rel (Delay (Force (Value v))) (MkTick (Value w))) ∧
 [exp_rel_Lam:]
   (∀s x y.
      exp_rel x y ⇒
@@ -768,7 +790,7 @@ Inductive exp_rel:
        v_rel (Recclosure f n) (Recclosure g n)) ∧
 [v_rel_Constructor:]
   (∀s vs ws.
-     LIST_REL (λv w. ∃n. thunk_rel n v w) vs ws ⇒
+     LIST_REL v_rel vs ws ⇒
        v_rel (Constructor s vs) (Constructor s ws)) ∧
 [v_rel_Thunk_Same:]
   (∀x y.
@@ -776,48 +798,13 @@ Inductive exp_rel:
      closed x ⇒
        v_rel (Thunk (INR x)) (Thunk (INR y))) ∧
 [v_rel_Thunk_Changed:]
-  (∀n v w.
-     thunk_rel n v w ⇒
-       v_rel (Thunk (INR (Force (Value v)))) w) ∧
+  (∀v w.
+     v_rel v w ⇒
+       v_rel (Thunk (INR (Force (Value v)))) (DoTick w)) ∧
 [v_rel_Atom:]
   (∀x.
-     v_rel (Atom x) (Atom x)) ∧
-[thunk_rel_Thunk_Changed:]
-  (∀n v w.
-     thunk_rel n v w ∧
-     is_thunky w ⇒
-       thunk_rel (SUC n) (Thunk (INR (Force (Value v)))) w) ∧
-[thunk_rel_Thunk_Same:]
-  (∀x y.
-     exp_rel x y ∧
-     closed x ⇒
-       thunk_rel 0 (Thunk (INR x)) (Thunk (INR y))) ∧
-[thunk_rel_Recclosure:]
-  (∀f g n.
-     LIST_REL (λ(fn,x) (gn,y).
-                 fn = gn ∧
-                 is_delay x ∧
-                 is_delay y ∧
-                 exp_rel x y ∧
-                 freevars x ⊆ set (MAP FST f)) f g ∧
-     is_thunky (Recclosure g n) ⇒
-       thunk_rel 0 (Recclosure f n) (Recclosure g n))
+     v_rel (Atom x) (Atom x))
 End
-
-Theorem thunk_rel_is_thunky:
-  ∀n v w. thunk_rel n v w ⇒ is_thunky v ∧ is_thunky w
-Proof
-  qsuff_tac ‘
-    (∀x y. exp_rel x y ⇒ T) ∧
-    (∀v w. v_rel v w ⇒ T) ∧
-    (∀n v w. thunk_rel n v w ⇒ is_thunky v ∧ is_thunky w)’
-  >- rw []
-  \\ ho_match_mp_tac exp_rel_strongind \\ rw []
-  \\ gvs [LIST_REL_EL_EQN, EVERY_MAP, EVERY_EL, ELIM_UNCURRY] \\ rw []
-  \\ first_x_assum (drule_then strip_assume_tac)
-  \\ first_x_assum (drule_then strip_assume_tac)
-  \\ gvs [Once exp_rel_cases]
-QED
 
 Theorem v_rel_def[simp]:
   (∀s x z.
@@ -837,7 +824,7 @@ Theorem v_rel_def[simp]:
   (∀s vs z.
      v_rel (Constructor s vs) z =
        (∃ws. z = Constructor s ws ∧
-             LIST_REL (λv w. ∃n. thunk_rel n v w) vs ws)) ∧
+             LIST_REL v_rel vs ws)) ∧
   (∀x z.
      v_rel (Atom x) z = (z = Atom x))
 Proof
@@ -852,13 +839,12 @@ Theorem v_rel_Thunk_def:
             (∀v. w ≠ Force (Value v)) ∧
             exp_rel w y ∧
             closed w) ∨
-     (∃n v. x = INR (Force (Value v)) ∧
-            thunk_rel n v z ∧
-            is_thunky z))
+     (∃v y. x = INR (Force (Value v)) ∧
+            z = DoTick y ∧
+            v_rel v y))
 Proof
   rw [Once exp_rel_cases]
-  \\ rw [EQ_SYM_EQ, AC CONJ_COMM CONJ_ASSOC, EQ_IMP_THM]
-  \\ rw [thunk_rel_is_thunky, SF SFY_ss, DISJ_EQ_IMP]
+  \\ rw [EQ_SYM_EQ, AC CONJ_COMM CONJ_ASSOC, EQ_IMP_THM, SF SFY_ss]
   \\ qpat_x_assum ‘exp_rel _ _’ mp_tac \\ rw [Once exp_rel_cases]
   \\ qpat_x_assum ‘exp_rel _ _’ mp_tac \\ rw [Once exp_rel_cases]
 QED
@@ -866,14 +852,19 @@ QED
 Theorem v_rel_Thunk_simps[simp]:
   (∀x s vs. ¬v_rel (Thunk x) (Constructor s vs)) ∧
   (∀x s y. ¬v_rel (Thunk x) (Closure s y)) ∧
-  (∀x y. ¬v_rel (Thunk x) (Atom y))
+  (∀x y. ¬v_rel (Thunk x) (Atom y)) ∧
+  (∀x w. ¬v_rel (DoTick x) w)
 Proof
   rpt conj_tac
   \\ Cases_on ‘x’ \\ rw [v_rel_Thunk_def]
-  \\ Cases_on ‘v’ \\ rw [Once exp_rel_cases]
+  \\ rw [Once exp_rel_cases]
 QED
 
 Theorem v_rel_rev[simp]:
+  (∀w.
+     v_rel v (DoTick w) =
+       (∃x. v = Thunk (INR (Force (Value x))) ∧
+            v_rel x w)) ∧
   (∀s y.
      v_rel v (Closure s y) =
        (∃x. v = Closure s x ∧
@@ -887,52 +878,25 @@ Theorem v_rel_rev[simp]:
                          is_delay x ∧
                          is_delay y ∧
                          exp_rel x y ∧
-                         freevars x ⊆ set (MAP FST f)) f g) ∨
-        (∃k w. v = Thunk (INR (Force (Value w))) ∧
-               thunk_rel k w (Recclosure g n) ∧
-               is_thunky (Recclosure g n)))) ∧
+                         freevars x ⊆ set (MAP FST f)) f g))) ∧
   (∀v s vs.
      v_rel v (Constructor s vs) =
        (∃ws. v = Constructor s ws ∧
-             LIST_REL (λv w. ∃n. thunk_rel n v w) ws vs)) ∧
+             LIST_REL v_rel ws vs)) ∧
+  (∀v s.
+     v_rel v (Thunk s) =
+      (∃x y.
+         v = Thunk (INR x) ∧
+         s = INR y ∧
+         exp_rel x y ∧
+         closed x ∧
+         (∀v. x ≠ Force (Value v)))) ∧
   (∀v a.
      v_rel v (Atom a) = (v = Atom a))
 Proof
   rw [] \\ Cases_on ‘v’ \\ simp []
   \\ rw [EQ_IMP_THM]
   \\ fs [v_rel_Thunk_def, SF SFY_ss]
-QED
-
-Theorem thunk_rel_def:
-  thunk_rel k v w ⇔
-    ((∃x y.
-        k = 0 ∧
-        v = Thunk (INR x) ∧
-        w = Thunk (INR y) ∧
-        (∀v. x ≠ Force (Value v)) ∧
-        closed x ∧
-        exp_rel x y) ∨
-     (∃j u.
-        k = SUC j ∧
-        v = Thunk (INR (Force (Value u))) ∧
-        thunk_rel j u w) ∨
-     (∃f g n.
-        k = 0 ∧
-        v = Recclosure f n ∧
-        w = Recclosure g n ∧
-        is_thunky w ∧
-        LIST_REL (λ(fn,x) (gn,y).
-                    fn = gn ∧
-                    is_delay x ∧
-                    is_delay y ∧
-                    exp_rel x y ∧
-                    freevars x ⊆ set (MAP FST f)) f g))
-Proof
-  rw [Once exp_rel_cases]
-  \\ rw [EQ_IMP_THM] \\ rw [DISJ_EQ_IMP]
-  \\ gs [thunk_rel_is_thunky, SF SFY_ss]
-  \\ qpat_x_assum ‘exp_rel _ _’ mp_tac \\ rw [Once exp_rel_cases]
-  \\ qpat_x_assum ‘exp_rel _ _’ mp_tac \\ rw [Once exp_rel_cases]
 QED
 
 Theorem is_delay_subst[local,simp]:
@@ -947,7 +911,7 @@ QED
 
 Theorem exp_rel_subst:
   ∀vs x ws y.
-    LIST_REL (λv w. ∃n. thunk_rel n v w) (MAP SND vs) (MAP SND ws) ∧
+    LIST_REL v_rel (MAP SND vs) (MAP SND ws) ∧
     MAP FST vs = MAP FST ws ∧
     exp_rel x y ⇒
       exp_rel (subst vs x) (subst ws y)
@@ -1010,9 +974,7 @@ Proof
   >- ((* Delay *)
     rw [Once exp_rel_cases] \\ simp [subst_def, exp_rel_Value, exp_rel_Delay,
                                      SF SFY_ss]
-    \\ ‘OPTREL (λv w. ∃n. thunk_rel n v w)
-               (ALOOKUP (REVERSE vs) v)
-               (ALOOKUP (REVERSE ws) v)’
+    \\ ‘OPTREL v_rel (ALOOKUP (REVERSE vs) v) (ALOOKUP (REVERSE ws) v)’
       suffices_by (rw [] \\ fs [subst_def, OPTREL_def, exp_rel_Var,
                                 exp_rel_Value, SF SFY_ss])
     \\ irule LIST_REL_OPTREL
@@ -1027,6 +989,8 @@ Proof
     \\ simp [subst_def]
     \\ irule exp_rel_Force \\ fs [])
   >- ((* Value *)
+    rw [Once exp_rel_cases])
+  >- ((* MkTick *)
     rw [Once exp_rel_cases])
 QED
 
@@ -1165,42 +1129,14 @@ Theorem exp_rel_exp_ok:
 Proof
   qsuff_tac ‘
     (∀x y. exp_rel x y ⇒ exp_ok x ⇒ exp_ok y) ∧
-    (∀v w. v_rel v w ⇒ v_ok v ⇒ v_ok w) ∧
-    (∀n v w. thunk_rel n v w ⇒ v_ok v ⇒ v_ok w)’
+    (∀v w. v_rel v w ⇒ v_ok v ⇒ v_ok w)’
   >- rw [SF SFY_ss]
   \\ ho_match_mp_tac exp_rel_strongind \\ rw []
   \\ gs [exp_ok_def, v_ok_def]
   \\ gs [LIST_REL_EL_EQN, EVERY_EL, EL_MAP, ELIM_UNCURRY]
   \\ gvs [MEM_EL, EL_MAP]
-  >- (
-    first_assum (irule_at Any)
-    \\ gs [EL_MAP])
-  >- (
-    rw []
-    \\ first_x_assum (drule_then strip_assume_tac)
-    \\ first_x_assum (drule_then strip_assume_tac))
-  >- (
-    first_assum (irule_at Any)
-    \\ gs [EL_MAP])
-QED
-
-Theorem thunk_rel_final:
-  (∀n u g s.
-     thunk_rel n u (Recclosure g s) ⇒
-       ∃f. thunk_rel 0 (Recclosure f s) (Recclosure g s)) ∧
-  (∀n u y.
-     thunk_rel n u (Thunk (INR y)) ⇒
-       ∃x. thunk_rel 0 (Thunk (INR x)) (Thunk (INR y)))
-Proof
-  conj_tac \\ Induct \\ rw []
-  \\ ((gvs [Once thunk_rel_def]
-       \\ gvs [Once thunk_rel_def]
-       \\ first_assum (irule_at Any)
-       \\ gs []
-       \\ NO_TAC) ORELSE
-      (gvs [Once thunk_rel_def]
-       \\ first_x_assum (irule_at Any)
-       \\ first_x_assum (irule_at Any)))
+  \\ first_assum (irule_at Any)
+  \\ gs [EL_MAP]
 QED
 
 Theorem exp_rel_eval_to:
@@ -1209,9 +1145,9 @@ Theorem exp_rel_eval_to:
     exp_inv x ∧
     exp_ok x ∧
     closed x ⇒
-      ∃j. ($= +++ (λv w. v_rel v w ∧ v_inv v ∧ v_ok v))
-            (eval_to (k + j) x)
-            (eval_to k y)
+      ($= +++ (λv w. v_rel v w ∧ v_inv v ∧ v_ok v))
+        (eval_to k x)
+        (eval_to k y)
 Proof
   ho_match_mp_tac eval_to_ind \\ rw []
   \\ qpat_x_assum ‘exp_rel _ _’ mp_tac
@@ -1223,159 +1159,39 @@ Proof
     \\ rw [eval_to_def] \\ gvs [exp_inv_def, exp_ok_def]
     \\ first_x_assum (drule_all_then strip_assume_tac)
     \\ first_x_assum (drule_all_then strip_assume_tac)
-    \\ map_every rename1 [
-      ‘exp_rel x1 x2’,
-      ‘exp_rel (Delay y) y2’,
-      ‘eval_to (j1 + k) (Delay y)’,
-      ‘eval_to (j2 + k) x1’]
-    \\ Cases_on ‘eval_to k x2 = INL Diverge’ \\ gs []
-    >- (
-      qexists_tac ‘j2’
-      \\ Cases_on ‘eval_to (k + j2) x1’ \\ gs [])
-    \\ ‘eval_to (j2 + k) x1 ≠ INL Diverge’
-      by (strip_tac
-          \\ drule_then assume_tac result_rel_Diverge_left
-          \\ gs [])
-    \\ drule_then (qspec_then ‘j1’ assume_tac) result_rel_mono_left \\ gs []
-    \\ ‘eval_to (j1 + k) (Delay y) ≠ INL Diverge’ by fs [eval_to_def]
-    \\ qpat_x_assum ‘_ (eval_to (j1 + k) (Delay _)) _’ assume_tac
-    \\ dxrule_then (qspec_then ‘j2’ assume_tac) result_rel_mono_left \\ gs []
-    \\ ‘∀j. eval_to (j + j2 + k) x1 = eval_to (j2 + k) x1’
-      by (strip_tac
-          \\ irule eval_to_mono \\ gs [])
-    \\ Cases_on ‘eval_to (j1 + j2 + k) x1’ \\ Cases_on ‘eval_to k x2’ \\ gvs []
-    >- (
-      qexists_tac ‘j1 + j2’
-      \\ simp [])
-    \\ Cases_on ‘eval_to (j1 + j2 + k) (Delay y)’
-    \\ Cases_on ‘eval_to k y2’ \\ gvs []
-    >- (
-      gs [eval_to_def])
-    \\ rename1 ‘eval_to _ x1 = INR v1’
-    \\ rename1 ‘eval_to _ x2 = INR v2’
-    \\ Cases_on ‘k = 0’ \\ gs []
-    >- (
-      Cases_on ‘dest_anyClosure v2’ \\ gs []
-      >- (
-        qexists_tac ‘j2’ \\ simp [eval_to_def]
-        \\ reverse (Cases_on ‘v1’) \\ Cases_on ‘v2’ \\ gvs [dest_anyClosure_def]
-        >- (
-          gs [CaseEqs ["option", "exp"]])
-        \\  qmatch_asmsub_abbrev_tac ‘LIST_REL _ f g’
-        \\ ‘OPTREL (λ_x _y. is_delay _x ∧ is_delay _y ∧ exp_rel _x _y)
-                   (ALOOKUP (REVERSE f) s) (ALOOKUP (REVERSE g) s)’
-          suffices_by (rw [] \\ gs [OPTREL_def]
-                       \\ qpat_x_assum `exp_rel _x _` mp_tac
-                       \\ rw [Once exp_rel_cases] \\ gs [])
-        \\ irule LIST_REL_OPTREL \\ gs []
-        \\ irule LIST_REL_mono
-        \\ first_assum (irule_at Any)
-        \\ simp [ELIM_UNCURRY])
-      \\ pairarg_tac \\ gvs []
-      \\ qexists_tac ‘0’
-      \\ Cases_on ‘eval_to 0 x1 = INL Diverge’ \\ gs []
-      \\ drule_then (qspec_then ‘j2’ (assume_tac o GSYM)) eval_to_mono
-      \\ gs [eval_to_def]
-      \\ reverse (Cases_on ‘v1’) \\ Cases_on ‘v2’ \\ gs [dest_anyClosure_def]
-      >- (
-        gs [CaseEqs ["option", "exp"], EVERY_EL]
-        \\ drule_then strip_assume_tac ALOOKUP_SOME_REVERSE_EL
-        \\ first_x_assum (drule_then strip_assume_tac) \\ gs [EL_MAP])
-      \\ qmatch_asmsub_abbrev_tac ‘LIST_REL _ f g’ \\ gvs []
-      \\ rename1 ‘ALOOKUP (REVERSE g) s1’
-      \\ ‘OPTREL (λ_x _y. is_delay _x ∧ is_delay _y ∧ exp_rel _x _y)
-                 (ALOOKUP (REVERSE f) s1) (ALOOKUP (REVERSE g) s1)’
-        suffices_by (rw [] \\ gs [OPTREL_def]
-                     \\ qpat_x_assum `exp_rel _x _` mp_tac
-                     \\ rw [Once exp_rel_cases] \\ gs [])
-      \\ irule LIST_REL_OPTREL \\ gs []
-      \\ irule LIST_REL_mono
-      \\ first_assum (irule_at Any)
-      \\ simp [ELIM_UNCURRY])
-    \\ simp [eval_to_def]
-    \\ Cases_on ‘dest_anyClosure v2’ \\ gs []
-    >- (
-      Q.REFINE_EXISTS_TAC ‘j + j2’ \\ simp []
-      \\ reverse (Cases_on ‘v1’) \\ Cases_on ‘v2’ \\ gvs [dest_anyClosure_def]
-      >- (
-        gs [CaseEqs ["option", "exp"], EVERY_EL])
-      \\ qmatch_asmsub_abbrev_tac ‘LIST_REL _ f g’ \\ gvs []
-      \\ rename1 ‘ALOOKUP (REVERSE g) s1’
-      \\ ‘OPTREL (λ_x _y. is_delay _x ∧ is_delay _y ∧ exp_rel _x _y)
-                 (ALOOKUP (REVERSE f) s1) (ALOOKUP (REVERSE g) s1)’
-        suffices_by (rw [] \\ gs [OPTREL_def]
-                     \\ qpat_x_assum `exp_rel _x _` mp_tac
-                     \\ rw [Once exp_rel_cases] \\ gs [])
-      \\ irule LIST_REL_OPTREL \\ gs []
-      \\ irule LIST_REL_mono
-      \\ first_assum (irule_at Any)
-      \\ simp [ELIM_UNCURRY])
-    \\ pairarg_tac \\ gvs []
-    \\ Cases_on ‘dest_anyClosure v1’ \\ gs []
-    >- (
-      reverse (Cases_on ‘v1’) \\ Cases_on ‘v2’ \\ gvs [dest_anyClosure_def]
-      >- (
-        gs [CaseEqs ["option", "exp"], EVERY_EL]
-        \\ drule_then strip_assume_tac ALOOKUP_SOME_REVERSE_EL
-        \\ gs [EL_MAP]
-        \\ first_x_assum (drule_then strip_assume_tac) \\ gs [])
-      \\ qmatch_asmsub_abbrev_tac ‘LIST_REL _ f g’ \\ gvs []
-      \\ rename1 ‘ALOOKUP (REVERSE g) s1’
-      \\ ‘OPTREL (λ_x _y. is_delay _x ∧ is_delay _y ∧ exp_rel _x _y)
-                 (ALOOKUP (REVERSE f) s1) (ALOOKUP (REVERSE g) s1)’
-        suffices_by (rw [] \\ gs [OPTREL_def]
-                     \\ qpat_x_assum `exp_rel _x _` mp_tac
-                     \\ rw [Once exp_rel_cases] \\ gs [])
-      \\ irule LIST_REL_OPTREL \\ gs []
-      \\ irule LIST_REL_mono
-      \\ first_assum (irule_at Any)
-      \\ simp [ELIM_UNCURRY])
-    \\ rename1 ‘dest_anyClosure v1 = INR vv’
-    \\ PairCases_on ‘vv’
-    \\ qmatch_goalsub_abbrev_tac ‘eval_to (k - 1) (subst binds1 body1)’
-    \\ qabbrev_tac ‘binds2 = vv2 ++ [vv0,Thunk (INR y)]’
-    \\ qabbrev_tac ‘body2 = vv1’
-    \\ ‘exp_rel (subst binds2 body2) (subst binds1 body1) ∧
-        exp_inv (subst binds2 body2) ∧
-        exp_ok (subst binds2 body2) ∧
-        closed (subst binds2 body2)’
-      by (unabbrev_all_tac
-          \\ irule_at Any exp_rel_subst
-          \\ irule_at Any exp_inv_subst
-          \\ irule_at Any exp_ok_subst
-          \\ gvs [closed_subst, eval_to_def]
-          \\ Cases_on ‘v1’ \\ Cases_on ‘v2’
-          \\ gvs [dest_anyClosure_def, v_rel_Thunk_def, v_ok_def]
-          >- (
-            irule_at Any thunk_rel_Thunk_Same \\ gs [])
-          >- (
-            irule_at Any thunk_rel_Thunk_Changed \\ gs []
-            \\ first_assum (irule_at Any))
-          \\ qmatch_asmsub_abbrev_tac ‘LIST_REL _ f g’ \\ gvs []
-          \\ rename1 ‘ALOOKUP (REVERSE g) s1’
-          \\ ‘OPTREL (λ_x _y. is_delay _x ∧ is_delay _y ∧ exp_rel _x _y)
-                  (ALOOKUP (REVERSE f) s1) (ALOOKUP (REVERSE g) s1)’
-            suffices_by (rw [] \\ gs [OPTREL_def]
-                         \\ qpat_x_assum `exp_rel _x _` mp_tac
-                         \\ rw [Once exp_rel_cases] \\ gs [])
-          \\ irule LIST_REL_OPTREL \\ gs []
-          \\ irule LIST_REL_mono
-          \\ first_assum (irule_at Any)
-          \\ simp [ELIM_UNCURRY])
-    \\ unabbrev_all_tac
-    \\ first_x_assum (drule_all_then strip_assume_tac)
-    \\ qmatch_asmsub_abbrev_tac ‘_ (eval_to _ e1) (eval_to _ e2)’
-    \\ Cases_on ‘eval_to (j + k - 1) e1 = INL Diverge’ \\ gs []
-    >- (
-      Cases_on ‘eval_to (j + k) x1 = INL Diverge’ \\ gs []
-      >- (
-        qexists_tac ‘j’ \\ simp [])
-      \\ ‘eval_to (j + k) x1 = eval_to (j2 + k) x1’
-        by (drule_then (qspec_then ‘j + k + j2’ assume_tac) eval_to_mono
-            \\ gs [])
-      \\ qexists_tac ‘j’ \\ simp [])
-    \\ drule_then (qspec_then ‘j2’ assume_tac) result_rel_mono_left
-    \\ qexists_tac ‘j2 + j’ \\ gs [])
+    \\ Cases_on ‘eval_to k x1’ \\ Cases_on ‘eval_to k g’ \\ gs []
+    \\ qpat_x_assum ‘exp_rel (Delay _) _’ mp_tac
+    \\ rw [Once exp_rel_cases] \\ gs [eval_to_def]
+    \\ pop_assum mp_tac
+    \\ rename1 ‘v_rel v1 v2’
+    \\ strip_tac
+    THEN (
+      Cases_on ‘v1’ \\ Cases_on ‘v2’ \\ gvs [dest_anyClosure_def]
+      >- ((* Thunk-Thunk *)
+        IF_CASES_TAC \\ gs []
+        \\ qmatch_goalsub_abbrev_tac ‘_ (eval_to _ (subst [s,w1] _))
+                                        (eval_to _ (subst [s,w2] _))’
+        \\ ‘[s,w1] = [] ++ [s,w1]’ by gs [] \\ pop_assum SUBST1_TAC
+        \\ ‘[s,w2] = [] ++ [s,w2]’ by gs [] \\ pop_assum SUBST1_TAC
+        \\ first_x_assum irule \\ simp []
+        \\ simp [closed_subst]
+        \\ irule_at Any exp_inv_subst
+        \\ irule_at Any exp_ok_subst
+        \\ irule_at Any exp_rel_subst \\ simp []
+        \\ unabbrev_all_tac \\ gs [v_ok_def]
+        \\ (irule_at Any v_rel_Thunk_Changed ORELSE
+            irule_at Any v_rel_Thunk_Same))
+      >- ((* Recclosure-Recclosure *)
+        rename1 ‘LIST_REL _ xs ys’
+        \\ ‘OPTREL (λ_x _y. is_delay _x ∧ is_delay _y ∧
+                            exp_rel _x _y)
+                   (ALOOKUP (REVERSE xs) s)
+                   (ALOOKUP (REVERSE ys) s)’
+          by (irule LIST_REL_OPTREL
+              \\ gs [LIST_REL_CONJ, ELIM_UNCURRY])
+        \\ gs [OPTREL_def]
+        \\ CASE_TAC \\ gs []
+        \\ CASE_TAC \\ gs [])))
   >- ((* Lam *)
     rw [Once exp_rel_cases, Once exp_inv_cases]
     \\ fs [exp_inv_def, eval_to_def, v_ok_def, exp_ok_def])
@@ -1385,129 +1201,26 @@ Proof
     \\ rename1 ‘exp_rel x1 x2’
     \\ rename1 ‘exp_rel y1 y2’
     \\ rw [eval_to_def]
-    >- ((* k = 0 *)
-      qexists_tac ‘0’
-      \\ simp [])
-    \\ first_x_assum (drule_all_then strip_assume_tac)
-    \\ first_x_assum (drule_all_then strip_assume_tac)
-    \\ rename1 ‘eval_to (j1 + k - 1) x1’
-    \\ rename1 ‘eval_to (j2 + k - 1) y1’
-    \\ Cases_on ‘eval_to (k - 1) x2 = INL Diverge’ \\ fs []
-    >- (
-      qexists_tac ‘j1’
-      \\ Cases_on ‘eval_to (j1 + k - 1) x1’ \\ gs [])
-    \\ ‘eval_to (j1 + k - 1) x1 ≠ INL Diverge’
-      by (strip_tac
-          \\ Cases_on ‘eval_to (k - 1) x2’ \\ gs [])
-    \\ ‘∀j. eval_to (j + j1 + k - 1) x1 = eval_to (j1 + k - 1) x1’
-      by (strip_tac
-          \\ drule_then (qspec_then ‘j + j1 + k - 1’ assume_tac) eval_to_mono
-          \\ gs [])
-    \\ Cases_on ‘eval_to (j1 + k - 1) x1’ \\ gs []
-    >- (
-      qexists_tac ‘j1’
-      \\ Cases_on ‘eval_to (k - 1) x2’ \\ gs [])
-    \\ Cases_on ‘eval_to (k - 1) x2’ \\ gs []
-    \\ Cases_on ‘eval_to (j2 + k - 1) y1 = INL Diverge’ \\ gs []
-    >- (
-      qexists_tac ‘j2’
-      \\ Cases_on ‘eval_to (j2 + k - 1) x1’ \\ gs []
-      \\ Cases_on ‘eval_to (j2 + k - 1) x1 = INL Diverge’ \\ gs []
-      \\ ‘eval_to (j2 + k - 1) x1 ≠ INL Diverge’ by fs []
-      \\ drule_then (qspec_then ‘j2 + (j1 + k) - 1’ assume_tac) eval_to_mono
-      \\ gs [])
-    \\ Q.REFINE_EXISTS_TAC ‘j + j1’ \\ simp []
-    \\ drule_then (qspec_then ‘j1’ assume_tac) result_rel_mono_left
-    \\ qexists_tac ‘j2’ \\ gs [])
+    \\ first_x_assum (drule_all_then assume_tac)
+    \\ first_x_assum (drule_all_then assume_tac)
+    \\ Cases_on ‘eval_to (k - 1) x1’ \\ Cases_on ‘eval_to (k - 1) x2’ \\ gs [])
   >- ((* Let SOME *)
     rw [Once exp_rel_cases])
   >- ((* If *)
     rw [Once exp_rel_cases] \\ fs [exp_inv_def, exp_ok_def]
     \\ rename1 ‘If x y z’
     \\ rw [eval_to_def] \\ gvs [exp_inv_def, exp_ok_def]
-    >- ((* k = 0 *)
-      qexists_tac ‘0’
-      \\ simp [])
     \\ first_x_assum (drule_then assume_tac) \\ fs []
     \\ first_x_assum (drule_then assume_tac) \\ fs []
     \\ first_x_assum (drule_then assume_tac) \\ fs []
-    \\ map_every rename1 [
-      ‘eval_to (j1 + k - 1) x’,
-      ‘eval_to (j2 + k - 1) y’,
-      ‘eval_to (j3 + k - 1) z’]
-    \\ Cases_on ‘eval_to (k - 1) x2 = INL Diverge’ \\ fs []
-    >- (
-      qexists_tac ‘j1’
-      \\ Cases_on ‘eval_to (j1 + k - 1) x’ \\ gs [])
-    \\ Cases_on ‘eval_to (k - 1) x2 = INL Type_error’ \\ fs []
-    >- (
-      qexists_tac ‘j1’ \\ simp []
-      \\ Cases_on ‘eval_to (j1 + k - 1) x’ \\ gs [])
-    \\ ‘∃res. eval_to (k - 1) x2 = INR res’
-      by (Cases_on ‘eval_to (k - 1) x2’ \\ fs []
-          \\ rename1 ‘eval_to (k - 1) x2 = INL err’
-          \\ Cases_on ‘err’ \\ gs [])
-    \\ ‘eval_to (j1 + k - 1) x ≠ INL Diverge’
-      by (strip_tac \\ gs [])
-    \\ qpat_x_assum ‘_ (eval_to _ x) (eval_to _ x2)’ assume_tac
-    \\ drule_then assume_tac result_rel_mono_left \\ gs []
-    \\ ‘∃res. eval_to (j1 + k - 1) x = INR res’
-      by (pop_assum (qspec_then ‘0’ assume_tac)
-          \\ Cases_on ‘eval_to (j1 + k - 1) x’ \\ gs [])
-    \\ IF_CASES_TAC \\ gvs []
-    >- ((* First branch taken *)
-      Cases_on ‘eval_to (k - 1) y2 = INL Diverge’ \\ gs []
-      >- (
-        Cases_on ‘eval_to (j2 + k - 1) y’ \\ gs []
-        \\ Cases_on ‘eval_to (j2 + k - 1) x = INL Diverge’ \\ gs []
-        >- (
-          qexists_tac ‘j2’ \\ simp [])
-        \\ ‘eval_to (j2 + k - 1) x = eval_to (j1 + k - 1) x’
-          by (drule_then (qspec_then ‘j1 + k - 1’ assume_tac) eval_to_mono
-              \\ ‘eval_to (j1 + k - 1) x ≠ INL Diverge’ by fs []
-              \\ drule_then (qspec_then ‘j2 + k - 1’ assume_tac) eval_to_mono
-              \\ Cases_on ‘j1 < j2’ \\ gs [])
-        \\ qexists_tac ‘j2’ \\ simp [])
-      \\ ‘eval_to (j2 + k - 1) y ≠ INL Diverge’
-        by (strip_tac
-            \\ Cases_on ‘eval_to (k - 1) y2’ \\ gs [])
-      \\ qpat_x_assum ‘_ (_ _ y) (_ _ y2)’ assume_tac
-      \\ drule_all_then (qspec_then ‘j1’ assume_tac) result_rel_mono_left
-      \\ first_x_assum (qspec_then ‘j2’ assume_tac)
-      \\ qexists_tac ‘j1 + j2’
-      \\ Cases_on ‘eval_to (j1 + j2 + k - 1) x’ \\ gs [])
-    \\ reverse IF_CASES_TAC \\ gvs []
-    >- (
-      qexists_tac ‘j1’ \\ simp []
-      \\ IF_CASES_TAC \\ gs []
-      \\ IF_CASES_TAC \\ gs [])
-        (* Second branch taken *)
-    \\ Cases_on ‘eval_to (k - 1) z2 = INL Diverge’ \\ gs []
-    >- (
-      Cases_on ‘eval_to (j3 + k - 1) z’ \\ gs []
-      \\ Cases_on ‘eval_to (j3 + k - 1) x = INL Diverge’ \\ gs []
-      >- (
-        qexists_tac ‘j3’ \\ simp [])
-      \\ ‘eval_to (j3 + k - 1) x = eval_to (j1 + k - 1) x’
-        by (drule_then (qspec_then ‘j1 + k - 1’ assume_tac) eval_to_mono
-            \\ ‘eval_to (j1 + k - 1) x ≠ INL Diverge’ by fs []
-            \\ drule_then (qspec_then ‘j3 + k - 1’ assume_tac) eval_to_mono
-            \\ Cases_on ‘j1 < j3’ \\ gs [])
-      \\ qexists_tac ‘j3’ \\ simp [])
-    \\ ‘eval_to (j3 + k - 1) z ≠ INL Diverge’
-      by (strip_tac
-          \\ Cases_on ‘eval_to (k - 1) z2’ \\ gs [])
-    \\ qpat_x_assum ‘_ (_ _ z) (_ _ z2)’ assume_tac
-    \\ drule_all_then (qspec_then ‘j1’ assume_tac) result_rel_mono_left
-    \\ first_x_assum (qspec_then ‘j3’ assume_tac)
-    \\ qexists_tac ‘j1 + j3’
-    \\ Cases_on ‘eval_to (j1 + j3 + k - 1) x’ \\ gs [])
+    \\ Cases_on ‘eval_to (k - 1) x’ \\ Cases_on ‘eval_to (k - 1) x2’ \\ gs []
+    \\ IF_CASES_TAC \\ gs []
+    \\ IF_CASES_TAC \\ gs []
+    \\ IF_CASES_TAC \\ gs []
+    \\ IF_CASES_TAC \\ gs [])
   >- ((* Letrec *)
     rw [Once exp_rel_cases]
     \\ rw [eval_to_def] \\ gvs [exp_inv_def, exp_ok_def]
-    >- ((* k = 0 *)
-      qexists_tac ‘0’
-      \\ simp [])
     \\ first_x_assum (irule_at Any)
     \\ fs [subst_funs_def, closed_def, freevars_subst, freevars_def]
     \\ fs [MAP_MAP_o, combinTheory.o_DEF, LAMBDA_PROD, SUBSET_DIFF_EMPTY,
@@ -1517,7 +1230,6 @@ Proof
     \\ gvs [MAP_MAP_o, combinTheory.o_DEF, EVERY2_MAP, LAMBDA_PROD,
             GSYM FST_THM]
     \\ irule_at Any LIST_EQ
-    \\ simp [Once thunk_rel_def]
     \\ gvs [EL_MAP, freevars_def, MAP_MAP_o, combinTheory.o_DEF]
     \\ drule_then assume_tac LIST_REL_LENGTH \\ simp []
     \\ irule_at Any exp_inv_subst
@@ -1532,1077 +1244,178 @@ Proof
     \\ gs [Once exp_rel_cases]
     \\ first_assum (irule_at Any) \\ gs [])
   >- ((* Delay *)
-    rw [Once exp_rel_cases] \\ gvs [exp_inv_def, eval_to_def, v_rel_Thunk_Same,
-                                    v_rel_Thunk_Changed, SF SFY_ss, v_ok_def,
-                                    exp_ok_def])
+    rw [Once exp_rel_cases] \\ gs [eval_to_def, exp_inv_def, exp_ok_def,
+                                   v_ok_def, v_rel_Thunk_Same])
   >- ((* Box *)
     rw [Once exp_rel_cases])
   >- ((* Force *)
     rw [Once exp_rel_cases]
     \\ rw [eval_to_def] \\ gs [exp_ok_def]
-    \\ Cases_on ‘∃s i xs. x = Prim (Proj s i) xs’ \\ gvs [exp_inv_def]
-    >- ((* Prim Proj *)
-      qpat_x_assum ‘exp_rel (Prim _ _) _’ mp_tac
-      \\ rw [Once exp_rel_cases]
-      \\ gs [Once exp_inv_cases]
-      \\ simp [eval_to_def]
-      \\ gvs [LIST_REL_EL_EQN]
-      \\ IF_CASES_TAC \\ fs []
-      \\ IF_CASES_TAC \\ fs []
-      >- ((* k = 0 *)
-        qexists_tac ‘0’
-        \\ simp [])
-      \\ gvs [LENGTH_EQ_NUM_compute, DECIDE “n < 1 ⇔ n = 0”, exp_inv_def]
-      \\ gs [exp_ok_def]
-      \\ rename1 ‘exp_rel x y’
-      \\ first_assum (qspec_then ‘[]’ mp_tac o CONV_RULE SWAP_FORALL_CONV)
-      \\ simp_tac list_ss [subst_funs_def, subst_empty]
-      \\ disch_then (drule_all_then (qx_choose_then ‘j’ assume_tac))
-      \\ Cases_on ‘eval_to (k - 1) y’ \\ gs []
-      >- (
-        qexists_tac ‘j’
-        \\ Cases_on ‘eval_to (j + k - 1) x’ \\ gs [])
-      \\ Cases_on ‘eval_to (j + k - 1) x’ \\ gs []
-      \\ rename1 ‘v_rel v1 v2’
-      \\ Cases_on ‘dest_Constructor v1’ \\ gs []
-      >- (
-        qexists_tac ‘j’
-        \\ Cases_on ‘v1’ \\ Cases_on ‘v2’ \\ gs [v_rel_Thunk_def])
-      \\ Cases_on ‘v1’ \\ Cases_on ‘v2’ \\ gs [LIST_REL_EL_EQN, v_rel_Thunk_def]
-      \\ reverse IF_CASES_TAC \\ gvs []
-      >- (
-        qexists_tac ‘j’ \\ gs []
-        \\ IF_CASES_TAC \\ gs [])
-      \\ rename1 ‘LENGTH f = LENGTH g’
-      \\ first_x_assum (drule_then (qx_choose_then ‘n’ assume_tac))
-      \\ drule_all_then assume_tac exp_rel_exp_ok
-      \\ drule_all_then assume_tac exp_ok_eval_to
-      \\ gs [EVERY_EL]
-      \\ rpt (first_x_assum (drule_all_then assume_tac)) \\ gvs []
-      \\ ‘∀m. eval_to (m + j + k - 1) x = eval_to (j + k - 1) x’
-        by (strip_tac \\ irule eval_to_mono \\ simp [])
-      \\ Cases_on ‘dest_anyThunk (EL i f)’ \\ gs []
-      >- (
-        gs [Once thunk_rel_def, dest_anyThunk_def]
-        \\ rename1 ‘LIST_REL _ f1 g1’
-        \\ rename1 ‘ALOOKUP (REVERSE g1) n1’
-        \\ gs [v_ok_def]
-        \\ ‘MEM n1 (MAP FST f1)’
-          by (gvs [EVERY_EL]
-              \\ first_x_assum (drule_then assume_tac)
-              \\ first_x_assum (drule_then assume_tac)
-              \\ gs [v_ok_def])
-        \\ ‘OPTREL (λ_x _y. is_delay _x ∧ is_delay _y ∧ exp_rel _x _y)
-                   (ALOOKUP (REVERSE f1) n1)
-                   (ALOOKUP (REVERSE g1) n1)’
-          suffices_by (rw []
-                       \\ gs [OPTREL_def, ALOOKUP_NONE, MAP_REVERSE]
-                       \\ CASE_TAC \\ gs [CaseEq "exp"])
-        \\ irule LIST_REL_OPTREL \\ gs []
-        \\ irule LIST_REL_mono
-        \\ first_assum (irule_at Any)
-        \\ rw [ELIM_UNCURRY])
-      \\ Cases_on ‘∃g1 n1. EL i g = Recclosure g1 n1’ \\ gs []
-      >- (
-        ‘MEM n1 (MAP FST g1)’
-          by (gvs [EVERY_EL, v_ok_def]
-              \\ first_x_assum (drule_then assume_tac)
-              \\ first_x_assum (drule_then assume_tac)
-              \\ gs [v_ok_def])
-        \\ simp [dest_anyThunk_def]
-        \\ Cases_on ‘ALOOKUP (REVERSE g1) n1’ \\ gs [ALOOKUP_NONE, MAP_REVERSE]
-        \\ rename1 ‘ALOOKUP (REVERSE g1) n1 = SOME v1’
-        \\ ‘∃x1. v1 = Delay x1’
-          by (drule_then (qx_choose_then ‘f1’ mp_tac)
-                (CONJUNCT1 thunk_rel_final)
-              \\ rw [Once thunk_rel_def]
-              \\ dxrule_then strip_assume_tac ALOOKUP_SOME_REVERSE_EL
-              \\ gvs [EVERY_EL, EL_MAP]
-              \\ first_x_assum (drule_then strip_assume_tac) \\ gs [])
-        \\ gvs [GSYM subst_funs_def]
-        \\ Cases_on ‘∃f1 m1. EL i f = Recclosure f1 m1’ \\ gs []
-        >- ((* Recclosure-Recclosure *)
-          gvs [Once thunk_rel_def]
-          \\ ‘OPTREL (λ_x _y. is_delay _x ∧ is_delay _y ∧ exp_rel _x _y)
-                     (ALOOKUP (REVERSE f1) m1)
-                     (ALOOKUP (REVERSE g1) m1)’
-            by (irule LIST_REL_OPTREL \\ gs []
-                \\ irule LIST_REL_mono
-                \\ first_assum (irule_at Any)
-                \\ rw [ELIM_UNCURRY])
-          \\ gs [OPTREL_def]
-          \\ ‘∃y1. _x = Delay y1’ by (Cases_on ‘_x’ \\ gs [])
-          \\ gvs [Once exp_rel_cases, dest_anyThunk_def]
-          \\ ‘exp_rel (subst_funs f1 y1) (subst_funs g1 x1) ∧
-              exp_inv (subst_funs f1 y1) ∧
-              exp_ok (subst_funs f1 y1) ∧
-              closed (subst_funs f1 y1)’
-            by (rw [subst_funs_def, closed_subst]
-                >- (
-                  irule_at Any exp_rel_subst
-                  \\ gvs [LIST_REL_EL_EQN, ELIM_UNCURRY, MAP_MAP_o,
-                          combinTheory.o_DEF, EVERY_MAP, EVERY_EL, GSYM FST_THM,
-                          SF ETA_ss]
-                  \\ irule_at Any LIST_EQ
-                  \\ rw [EL_MAP, Once thunk_rel_def, EVERY_EL, LIST_REL_EL_EQN,
-                         ELIM_UNCURRY])
-                >- (
-                  irule_at Any exp_inv_subst
-                  \\ gvs [LIST_REL_EL_EQN, ELIM_UNCURRY, MAP_MAP_o,
-                          combinTheory.o_DEF, EVERY_MAP, thunk_inv_def,
-                          EVERY_EL]
-                  \\ dxrule_then strip_assume_tac ALOOKUP_SOME_REVERSE_EL
-                  \\ gvs []
-                  \\ first_x_assum (drule_then strip_assume_tac) \\ gs [])
-                >- (
-                  irule_at Any exp_ok_subst
-                  \\ gvs [LIST_REL_EL_EQN, ELIM_UNCURRY, MAP_MAP_o,
-                          combinTheory.o_DEF, EVERY_MAP, v_ok_def, EVERY_EL]
-                  \\ dxrule_then strip_assume_tac ALOOKUP_SOME_REVERSE_EL
-                  \\ gvs [] \\ rw []
-                  \\ last_x_assum (drule_then assume_tac)
-                  \\ gs [v_ok_def, EVERY_EL, EL_MAP]
-                  \\ first_x_assum (drule_then assume_tac)
-                  \\ gvs [exp_ok_def]
-                  \\ qpat_x_assum ‘∀m. n < LENGTH g1 ⇒ _ ∧ _’
-                    (drule_then assume_tac)
-                  \\ gs []
-                  \\ pop_assum (SUBST1_TAC o SYM)
-                  \\ irule MEM_MAP_f
-                  \\ gs [MEM_EL]
-                  \\ irule_at Any EQ_REFL \\ gs [])
-                >- (
-                  gvs [LIST_REL_EL_EQN, ELIM_UNCURRY, MAP_MAP_o,
-                       combinTheory.o_DEF, SF ETA_ss]
-                  \\ dxrule_then strip_assume_tac ALOOKUP_SOME_REVERSE_EL
-                  \\ gvs []
-                  \\ first_x_assum (drule_then strip_assume_tac)
-                  \\ gs [freevars_def]))
-          \\ first_x_assum (drule_all_then (qx_choose_then ‘j1’ assume_tac))
-          \\ Cases_on ‘eval_to (k - 1) (subst_funs g1 x1) = INL Diverge’
-          >- (
-            Cases_on ‘eval_to (k - 1) x = INL Diverge’ \\ gs []
-            >- (
-              qexists_tac ‘0’
-              \\ simp [])
-            \\ ‘∀m. eval_to (m + k - 1) x = eval_to (j + k - 1) x’
-              by (rw []
-                  \\ drule_then (qspec_then ‘m + k - 1’ assume_tac) eval_to_mono
-                  \\ drule_then (qspec_then ‘j + k - 1’ assume_tac) eval_to_mono
-                  \\ gs [])
-            \\ simp []
-            \\ first_assum (irule_at Any))
-          \\ Q.REFINE_EXISTS_TAC ‘m + j’ \\ simp []
-          \\ drule_then (qspec_then ‘j’ assume_tac) result_rel_mono_right
-          \\ qexists_tac ‘j1’ \\ gs [])
-          (* lhs is thunk *)
-        \\ gvs [Once thunk_rel_def]
-        \\ rename1 ‘thunk_rel n u _’
-        \\ last_x_assum assume_tac
-        \\ gvs [exp_inv_def, dest_anyThunk_def, v_ok_def, EVERY_EL]
-        \\ Cases_on ‘eval_to (k - 1) (subst_funs g1 x1) = INL Diverge’
-        >- (
-          Cases_on ‘eval_to (k - 1) x = INL Diverge’ \\ gs []
-          >- (
-            qexists_tac ‘0’
-            \\ simp [])
-          \\ ‘∀m. eval_to (m + k - 1) x = eval_to (j + k - 1) x’
-            by (rw []
-                \\ drule_then (qspec_then ‘m + k - 1’ assume_tac) eval_to_mono
-                \\ drule_then (qspec_then ‘j + k - 1’ assume_tac) eval_to_mono
-                \\ gs [])
-          \\ simp [Once subst_funs_def]
-          \\ ‘v_ok u’
-            by (gs [EVERY_EL, v_ok_def]
-                \\ last_x_assum (drule_then strip_assume_tac)
-                \\ gs [v_ok_def, exp_ok_def])
-          \\ pop_assum mp_tac
-          \\ qpat_x_assum ‘thunk_inv _’ mp_tac
-          \\ qpat_x_assum ‘thunk_rel _ _ _’ mp_tac
-          \\ ntac 4 (last_x_assum kall_tac)
-          \\ last_x_assum assume_tac
-          \\ ntac 10 (last_x_assum kall_tac)
-          \\ qid_spec_tac ‘u’
-          \\ qid_spec_tac ‘n’
-          \\ Induct
-          >- (
-            rw [Once thunk_rel_def]
-            \\ gs [v_ok_def, thunk_inv_def, eval_to_def, dest_anyThunk_def]
-            \\ CASE_TAC \\ gs [ALOOKUP_NONE, MAP_REVERSE]
-            \\ drule_then (qspec_then ‘REVERSE g1’ mp_tac) ALOOKUP_SOME_EL_2
-            \\ simp [MAP_REVERSE]
-            \\ impl_keep_tac
-            >- (
-              irule LIST_EQ
-              \\ gvs [LIST_REL_EL_EQN]
-              \\ rw [EL_MAP]
-              \\ first_x_assum (drule_then assume_tac)
-              \\ gs [ELIM_UNCURRY])
-            \\ strip_tac
-            \\ gvs [EL_REVERSE, LIST_REL_EL_EQN]
-            \\ qmatch_asmsub_abbrev_tac ‘EL m f’
-            \\ ‘m < LENGTH g1’ by fs [Abbr ‘m’]
-            \\ first_assum (drule_then assume_tac)
-            \\ rpt (pairarg_tac \\ fs []) \\ gvs []
-            \\ CASE_TAC \\ gs []
-            \\ Cases_on ‘k ≤ 1’ \\ gs []
-            >- (
-              qexists_tac ‘0’
-              \\ simp [])
-            \\ Q.REFINE_EXISTS_TAC ‘z + 1’ \\ simp []
-            \\ once_rewrite_tac [arithmeticTheory.ADD_COMM]
-            \\ qpat_x_assum ‘_ = INL Diverge’ (SUBST1_TAC o SYM)
-            \\ last_x_assum (irule_at Any)
-            \\ simp [subst_funs_def, closed_subst]
-            \\ irule_at Any exp_rel_subst
-            \\ irule_at Any exp_inv_subst
-            \\ irule_at Any exp_ok_subst
-            \\ irule_at Any LIST_EQ
-            \\ gvs [LIST_REL_EL_EQN, ELIM_UNCURRY, MAP_MAP_o, v_ok_def,
-                    combinTheory.o_DEF, EVERY_MAP, EVERY_EL, GSYM FST_THM,
-                    thunk_inv_def, SF ETA_ss]
-            \\ gvs [Once exp_rel_cases, freevars_def]
-            \\ first_x_assum (drule_then assume_tac) \\ gs [exp_ok_def]
-            \\ first_x_assum (drule_then strip_assume_tac) \\ gvs []
-            \\ csimp [EL_MAP, Once thunk_rel_def, EVERY_EL, ELIM_UNCURRY,
-                      LIST_REL_EL_EQN]
-            \\ rw []
-            \\ irule MEM_MAP_f
-            \\ rw [EL_MEM])
-          \\ rw [Once thunk_rel_def]
-          \\ rw [eval_to_def, dest_anyThunk_def]
-          \\ Cases_on ‘k ≤ 1’ \\ gs []
-          >- (
-            qexists_tac ‘0’
-            \\ simp [])
-          \\ simp [Once subst_funs_def]
-          \\ Q.REFINE_EXISTS_TAC ‘m + 1’
-          \\ simp []
-          \\ once_rewrite_tac [arithmeticTheory.ADD_COMM]
-          \\ first_x_assum (irule_at Any)
-          \\ gs [thunk_inv_def, v_ok_def, exp_inv_def, exp_ok_def])
-      \\ Q.REFINE_EXISTS_TAC ‘m + j’
-      \\ simp [Once subst_funs_def]
-      \\ ‘v_ok u’
-        by (gs [EVERY_EL, v_ok_def]
-            \\ last_x_assum (drule_then strip_assume_tac)
-            \\ gs [v_ok_def, exp_ok_def])
-      \\ pop_assum mp_tac
-      \\ qpat_x_assum ‘thunk_inv _’ mp_tac
-      \\ qpat_x_assum ‘thunk_rel _ _ _’ mp_tac
-      \\ ntac 4 (last_x_assum kall_tac)
-      \\ last_x_assum assume_tac
-      \\ ntac 10 (last_x_assum kall_tac)
-      \\ qid_spec_tac ‘u’
-      \\ qid_spec_tac ‘n’
-      \\ Induct
-      >- (
-        rw [Once thunk_rel_def]
-        \\ gs [v_ok_def, thunk_inv_def, eval_to_def, dest_anyThunk_def]
-        \\ CASE_TAC \\ gs [ALOOKUP_NONE, MAP_REVERSE]
-        \\ drule_then (qspec_then ‘REVERSE g1’ mp_tac) ALOOKUP_SOME_EL_2
-        \\ simp [MAP_REVERSE]
-        \\ impl_keep_tac
-        >- (
-          irule LIST_EQ
-          \\ gvs [LIST_REL_EL_EQN]
-          \\ rw [EL_MAP]
-          \\ first_x_assum (drule_then assume_tac)
-          \\ gs [ELIM_UNCURRY])
-        \\ strip_tac
-        \\ gvs [EL_REVERSE, LIST_REL_EL_EQN]
-        \\ qmatch_asmsub_abbrev_tac ‘EL m f’
-        \\ ‘m < LENGTH g1’ by fs [Abbr ‘m’]
-        \\ first_assum (drule_then assume_tac)
-        \\ rpt (pairarg_tac \\ fs []) \\ gvs []
-        \\ CASE_TAC \\ gs []
-        \\ Q.REFINE_EXISTS_TAC ‘z + 1’ \\ simp []
-        \\ rename1 ‘subst_funs f1 y1’
-        \\ ‘exp_rel (subst_funs f1 y1) (subst_funs g1 x1) ∧
-            exp_inv (subst_funs f1 y1) ∧
-            exp_ok (subst_funs f1 y1) ∧
-            closed (subst_funs f1 y1)’
-          by (
-            simp [subst_funs_def, closed_subst]
-            \\ irule_at Any exp_rel_subst
-            \\ irule_at Any exp_inv_subst
-            \\ irule_at Any exp_ok_subst
-            \\ irule_at Any LIST_EQ
-            \\ gvs [LIST_REL_EL_EQN, ELIM_UNCURRY, MAP_MAP_o, v_ok_def,
-                    combinTheory.o_DEF, EVERY_MAP, EVERY_EL, GSYM FST_THM,
-                    thunk_inv_def, SF ETA_ss]
-            \\ gvs [Once exp_rel_cases, freevars_def]
-            \\ first_x_assum (drule_then assume_tac) \\ gs [exp_ok_def]
-            \\ first_x_assum (drule_then strip_assume_tac) \\ gvs []
-            \\ csimp [EL_MAP, Once thunk_rel_def, EVERY_EL, ELIM_UNCURRY,
-                      LIST_REL_EL_EQN]
-            \\ rw []
-            \\ irule MEM_MAP_f
-            \\ rw [EL_MEM])
-        \\ first_x_assum (drule_all_then (qx_choose_then ‘j1’ assume_tac))
-        \\ drule_then (qspec_then ‘j’ assume_tac) result_rel_mono_right
-        \\ qexists_tac ‘j1’ \\ gs [])
-      \\ rw [Once thunk_rel_def]
-      \\ rw [eval_to_def, dest_anyThunk_def]
-      \\ Q.REFINE_EXISTS_TAC ‘m + 1’
-      \\ simp [Once subst_funs_def]
-      \\ gs [thunk_inv_def, v_ok_def, exp_inv_def, exp_ok_def])
-    \\ Cases_on ‘∃x1. EL i g = Thunk (INR x1)’ \\ gs []
-    >- (
-      simp [dest_anyThunk_def]
-      \\ last_x_assum
-        (qspec_then ‘[]’ assume_tac o CONV_RULE SWAP_FORALL_CONV)
-      \\ gvs [subst_funs_def, Once thunk_rel_def]
-      >- ((* lhs is the same thunk *)
-        Cases_on ‘eval_to (k - 1) x1 = INL Diverge’
-        >- (
-          Cases_on ‘eval_to (k - 1) x = INL Diverge’ \\ gs []
-          >- (
-            qexists_tac ‘0’
-            \\ simp [])
-          \\ ‘∀m. eval_to (m + k - 1) x = eval_to (j + k - 1) x’
-            by (rw []
-                \\ drule_then (qspec_then ‘m + k - 1’ assume_tac) eval_to_mono
-                \\ drule_then (qspec_then ‘j + k - 1’ assume_tac) eval_to_mono
-                \\ gs [])
-          \\ simp []
-          \\ qpat_x_assum ‘_ = INL Diverge’ (SUBST1_TAC o SYM)
-          \\ first_x_assum (irule_at Any)
-          \\ gs [v_ok_def, EVERY_EL]
-          \\ first_x_assum (drule_then assume_tac)
-          \\ first_x_assum (drule_then assume_tac)
-          \\ gs [v_ok_def])
-        \\ Q.REFINE_EXISTS_TAC ‘m + j’ \\ simp []
-        \\ rename1 ‘exp_rel x0 x1’
-        \\ ‘exp_ok x0’
-          by (gs [v_ok_def, EVERY_EL]
-              \\ last_x_assum (drule_then assume_tac)
-              \\ gs [v_ok_def])
-        \\ first_x_assum (drule_all_then (qx_choose_then ‘j1’ assume_tac))
-        \\ drule_then (qspec_then ‘j’ assume_tac) result_rel_mono_right
-        \\ qexists_tac ‘j1’ \\ gs [])
-          (* lhs is another thunk *)
-        \\ rename1 ‘thunk_rel n u _’
-        \\ gvs [exp_inv_def, dest_anyThunk_def, v_ok_def, EVERY_EL]
-        \\ Cases_on ‘eval_to (k - 1) x1 = INL Diverge’
-        >- (
-          Cases_on ‘eval_to (k - 1) x = INL Diverge’ \\ gs []
-          >- (
-            qexists_tac ‘0’
-            \\ simp [])
-          \\ ‘∀m. eval_to (m + k - 1) x = eval_to (j + k - 1) x’
-            by (rw []
-                \\ drule_then (qspec_then ‘m + k - 1’ assume_tac) eval_to_mono
-                \\ drule_then (qspec_then ‘j + k - 1’ assume_tac) eval_to_mono
-                \\ gs [])
-          \\ simp [Once subst_funs_def]
-        \\ ‘v_ok u’
-          by (gs [EVERY_EL, v_ok_def]
-              \\ last_x_assum (drule_then strip_assume_tac)
-              \\ gs [v_ok_def, exp_ok_def])
-        \\ pop_assum mp_tac
-        \\ qpat_x_assum ‘thunk_inv _’ mp_tac
-        \\ qpat_x_assum ‘thunk_rel _ _ _’ mp_tac
-        \\ ntac 4 (last_x_assum kall_tac)
-        \\ last_x_assum assume_tac
-        \\ ntac 10 (last_x_assum kall_tac)
-        \\ qid_spec_tac ‘u’
-        \\ qid_spec_tac ‘n’
-        \\ Induct
-        >- (
-          rw [Once thunk_rel_def]
-          \\ gs [v_ok_def, thunk_inv_def, eval_to_def, dest_anyThunk_def]
-          \\ Cases_on ‘k ≤ 1’ \\ gs []
-          >- (
-            qexists_tac ‘0’
-            \\ simp [])
-          \\ Q.REFINE_EXISTS_TAC ‘m + 1’ \\ simp [subst_funs_def]
-          \\ once_rewrite_tac [arithmeticTheory.ADD_COMM]
-          \\ qpat_x_assum ‘_ = INL Diverge’ (SUBST1_TAC o SYM)
-          \\ last_x_assum (irule_at Any) \\ gs [])
-        \\ rw [Once thunk_rel_def]
-        \\ rw [eval_to_def, dest_anyThunk_def]
-        \\ Cases_on ‘k ≤ 1’ \\ gs []
-        >- (
-          qexists_tac ‘0’
-          \\ simp [])
-        \\ simp [Once subst_funs_def]
-        \\ Q.REFINE_EXISTS_TAC ‘m + 1’ \\ simp []
-        \\ once_rewrite_tac [arithmeticTheory.ADD_COMM]
-        \\ first_x_assum (irule_at Any)
-        \\ gs [thunk_inv_def, v_ok_def, exp_inv_def, exp_ok_def])
-      \\ Q.REFINE_EXISTS_TAC ‘m + j’
-      \\ simp [Once subst_funs_def]
-      \\ ‘v_ok u’
-        by (gs [EVERY_EL, v_ok_def]
-            \\ last_x_assum (drule_then strip_assume_tac)
-            \\ gs [v_ok_def, exp_ok_def])
-      \\ pop_assum mp_tac
-      \\ qpat_x_assum ‘thunk_inv _’ mp_tac
-      \\ qpat_x_assum ‘thunk_rel _ _ _’ mp_tac
-      \\ ntac 4 (last_x_assum kall_tac)
-      \\ last_x_assum assume_tac
-      \\ ntac 10 (last_x_assum kall_tac)
-      \\ qid_spec_tac ‘u’
-      \\ qid_spec_tac ‘n’
-      \\ Induct
-      >- (
-        rw [Once thunk_rel_def]
-        \\ gs [v_ok_def, thunk_inv_def, eval_to_def, dest_anyThunk_def]
-        \\ Q.REFINE_EXISTS_TAC ‘m + 1’ \\ simp [subst_funs_def]
-        \\ first_x_assum (drule_all_then (qx_choose_then ‘j1’ assume_tac))
-        \\ drule_then (qspec_then ‘j’ assume_tac) result_rel_mono_right
-        \\ qexists_tac ‘j1’ \\ gs [])
-      \\ rw [Once thunk_rel_def]
-      \\ rw [eval_to_def, dest_anyThunk_def]
-      \\ Q.REFINE_EXISTS_TAC ‘m + 1’
-      \\ simp [Once subst_funs_def]
-      \\ gs [thunk_inv_def, v_ok_def, exp_inv_def, exp_ok_def])
-    \\ ‘F’ suffices_by rw []
-    \\ drule_then strip_assume_tac thunk_rel_is_thunky
-    \\ Cases_on ‘EL i f’ \\ Cases_on ‘EL i g’ \\ gs [dest_anyThunk_def]
-    \\ rename1 ‘ss ≠ INR _’
-    \\ Cases_on ‘ss’ \\ gs [])
     \\ rename1 ‘exp_rel x y’
-    \\ first_x_assum (drule_then assume_tac) \\ gs []
-    \\ Cases_on ‘eval_to k y’ \\ fs []
-    >- (
-      qexists_tac ‘j’
-      \\ Cases_on ‘eval_to (j + k) x’ \\ gs [])
-    \\ Cases_on ‘eval_to (j + k) x’ \\ gs []
+    \\ first_x_assum (drule_then assume_tac)
+    \\ Cases_on ‘∃s i xs. x = Prim (Proj s i) xs’ \\ gvs [exp_inv_def]
+    >- cheat
+    \\ Cases_on ‘eval_to k x’ \\ Cases_on ‘eval_to k y’ \\ gs []
+    \\ pairarg_tac \\ gvs []
+    \\ pairarg_tac \\ gvs []
     \\ rename1 ‘v_rel v1 v2’
-    \\ Cases_on ‘∃z. v2 = Thunk (INR z)’ \\ gvs []
-    >- ((* rhs is thunk *)
-      Cases_on ‘v1’ \\ gs []
-      \\ rename1 ‘v_rel (Thunk s1) _’ \\ Cases_on ‘s1’ \\ gs []
-      \\ gvs [v_rel_Thunk_def, v_ok_def]
-      >- ((* Thunk - Thunk *)
-        Cases_on ‘k = 0’ \\ gs []
-        >- (
-          qexists_tac ‘0’
-          \\ Cases_on ‘eval_to 0 x = INL Diverge’ \\ gs []
-          >- (
-            simp [dest_anyThunk_def])
-          \\ ‘eval_to 0 x = eval_to j x’
-            by (once_rewrite_tac [EQ_SYM_EQ]
-                \\ irule eval_to_mono
-                \\ simp [])
-          \\ simp [dest_anyThunk_def])
-        \\ first_x_assum
-          (qspec_then ‘[]’ assume_tac o CONV_RULE SWAP_FORALL_CONV)
-        \\ gs [subst_funs_def]
-        \\ first_x_assum (drule_all_then strip_assume_tac)
-        \\ rename1 ‘_ (eval_to (j1 + k - 1) z1)’
-        \\ Cases_on ‘eval_to (j1 + k - 1) z1 = INL Diverge’ \\ gs []
-        >- (
-          Cases_on ‘eval_to (j1 + k) x = INL Diverge’ \\ gs []
-          >- (
-            qexists_tac ‘j1’
-            \\ simp [dest_anyThunk_def])
-          \\ ‘eval_to (j1 + k) x = eval_to (j + k) x’
-            by (drule_then (qspec_then ‘j + k’ assume_tac) eval_to_mono
-                \\ ‘eval_to (j + k) x ≠ INL Diverge’ by fs []
-                \\ drule_then (qspec_then ‘j1 + k’ assume_tac) eval_to_mono
-                \\ Cases_on ‘j ≤ j1’ \\ gs [])
-          \\ qexists_tac ‘j1’
-          \\ simp [dest_anyThunk_def])
-        \\ drule_all_then (qspec_then ‘j’ assume_tac) result_rel_mono_left
-        \\ ‘eval_to (j1 + j + k) x = eval_to (j + k) x’
-          by (irule eval_to_mono
-              \\ simp [])
-        \\ qexists_tac ‘j1 + j’
-        \\ gs [dest_anyThunk_def])
-      \\ Cases_on ‘k = 0’ \\ simp []
-      >- (
-        qexists_tac ‘0’
-        \\ Cases_on ‘eval_to 0 x = INL Diverge’ \\ gs []
-        >- (
-          simp [dest_anyThunk_def])
-        \\ ‘eval_to 0 x = eval_to j x’
-          by (once_rewrite_tac [EQ_SYM_EQ]
-              \\ irule eval_to_mono
-              \\ simp [])
-        \\ simp [dest_anyThunk_def])
-      \\ ‘∀m. eval_to (m + j + k) x = eval_to (j + k) x’
-        by (strip_tac
-            \\ irule eval_to_mono
-            \\ simp [])
-      \\ first_x_assum (qspec_then ‘[]’ assume_tac o CONV_RULE SWAP_FORALL_CONV)
-      \\ gs [dest_anyThunk_def, subst_funs_def]
-      \\ Cases_on ‘eval_to (k - 1) z = INL Diverge’ \\ gs []
-      >- (
-        qexists_tac ‘0’
-        \\ Cases_on ‘eval_to k x = INL Diverge’ \\ gs []
-        \\ ‘eval_to k x = eval_to (j + k) x’
-          by (once_rewrite_tac [EQ_SYM_EQ]
-              \\ irule eval_to_mono
-              \\ simp [])
-        \\ gs [exp_inv_def]
-        \\ ntac 5 (last_x_assum kall_tac)
-        \\ gs [exp_ok_def]
-        \\ map_every (fn tm => qpat_x_assum tm kall_tac) [
-          ‘eval_to k y = _’,
-          ‘eval_to (j + k) x = _’,
-          ‘∀m. eval_to _ _ = _’,
-          ‘eval_to k x = _’ ]
-        \\ qpat_x_assum ‘v_ok v’ mp_tac
-        \\ qpat_x_assum ‘thunk_rel _ _ _’ mp_tac
-        \\ qpat_x_assum  ‘thunk_inv v’ mp_tac
-        \\ qid_spec_tac ‘v’
-        \\ Induct_on ‘n’
-        >- (
-          rw [Once thunk_rel_def]
-          \\ gs [exp_inv_def, v_ok_def]
-          \\ first_x_assum (drule_all_then strip_assume_tac)
-          \\ gs [eval_to_def, dest_anyThunk_def, subst_funs_def]
-          \\ IF_CASES_TAC \\ gs []
-          \\ rename1 ‘eval_to (j + k - 1) x’
-          \\ Cases_on ‘eval_to (k - 2) x = INL Diverge’ \\ gs []
-          \\ drule_then (qspec_then ‘k - 2 + j + 1’ assume_tac) eval_to_mono
-          \\ gs [])
-        \\ rw [Once thunk_rel_def]
-        \\ fs [thunk_inv_def, exp_inv_def, v_ok_def, exp_ok_def]
-        \\ first_x_assum (drule_all_then assume_tac)
-        \\ simp [eval_to_def, dest_anyThunk_def]
-        \\ IF_CASES_TAC \\ gs [subst_funs_def]
-        \\ Cases_on ‘eval_to (k - 2) (Force (Value u)) = INL Diverge’ \\ gs []
-        \\ drule_then (qspec_then ‘k - 1’ assume_tac) eval_to_mono \\ gs [])
-      \\ Q.REFINE_EXISTS_TAC ‘m + j’
-      \\ gs [exp_inv_def, exp_ok_def]
-      \\ ntac 5 (last_x_assum kall_tac)
-      \\ map_every (fn tm => qpat_x_assum tm kall_tac) [
-        ‘eval_to k y = _’,
-        ‘eval_to (j + k) x = _’,
-        ‘∀m. eval_to _ _ = _’ ]
-      \\ qpat_x_assum ‘v_ok v’ mp_tac
-      \\ qpat_x_assum ‘thunk_rel _ _ _’ mp_tac
-      \\ qpat_x_assum ‘thunk_inv v’ mp_tac
-      \\ qid_spec_tac ‘v’
-      \\ Induct_on ‘n’
-      >- (
-        rw [Once thunk_rel_def]
-        \\ gs [exp_inv_def, v_ok_def, exp_ok_def]
-        \\ first_x_assum (drule_all_then strip_assume_tac)
-        \\ gs [eval_to_def, dest_anyThunk_def, subst_funs_def]
-        \\ rename1 ‘eval_to (j1 + k - 1) x’
-        \\ qexists_tac ‘j1 + 1’ \\ gs []
-        \\ ‘eval_to (j1 + k - 1) x ≠ INL Diverge’
-          by (strip_tac
-              \\ Cases_on ‘eval_to (k - 1) z’ \\ gs [])
-        \\ dxrule_then (qspec_then ‘j’ assume_tac) result_rel_mono_left
-        \\ gs [])
-      \\ rw [Once thunk_rel_def]
-      \\ fs [thunk_inv_def, exp_inv_def, exp_ok_def, v_ok_def]
-      \\ first_x_assum (drule_all_then strip_assume_tac)
-      \\ simp [eval_to_def, dest_anyThunk_def]
-      \\ qexists_tac ‘m + 1’ \\ gs [subst_funs_def])
-    \\ Cases_on ‘∃g n. v2 = Recclosure g n’ \\ gvs []
-    >- ((* Recclosure - Recclosure *)
-      rename1 ‘LIST_REL _ f g’
-      \\ Cases_on ‘dest_anyThunk (Recclosure g n)’ \\ gs []
-      >- (
-        qexists_tac ‘j’
-        \\ gs [dest_anyThunk_def]
-        \\ rename1 ‘ALOOKUP (REVERSE f) s’
-        \\ ‘OPTREL (λ_x _y. is_delay _x ∧ is_delay _y ∧ exp_rel _x _y)
-                   (ALOOKUP (REVERSE f) s) (ALOOKUP (REVERSE g) s)’
-          suffices_by (rw [] \\ gs [OPTREL_def]
-                       \\ qpat_x_assum `exp_rel _x _` mp_tac
-                       \\ rw [Once exp_rel_cases] \\ gs [])
-        \\ irule LIST_REL_OPTREL \\ gs []
-        \\ irule LIST_REL_mono
-        \\ first_assum (irule_at Any)
-        \\ simp [ELIM_UNCURRY])
-      \\ Cases_on ‘k = 0’ \\ gs []
-      >- (
-        qexists_tac ‘0’
-        \\ Cases_on ‘eval_to 0 x = INL Diverge’ \\ gs []
-        >- (
-          gvs [dest_anyThunk_def, CaseEqs ["option", "exp"]])
-        \\ ‘eval_to 0 x = eval_to j x’
-          by (once_rewrite_tac [EQ_SYM_EQ]
-              \\ irule eval_to_mono
-              \\ simp [])
-        \\ gs []
-        \\ pairarg_tac \\ gvs [dest_anyThunk_def, CaseEqs ["option", "exp"]]
-        \\ qmatch_asmsub_rename_tac ‘ALOOKUP (REVERSE g) s’
-        >- (
-          ‘OPTREL (λ_x _y. is_delay _x ∧ is_delay _y ∧ exp_rel _x _y)
-                     (ALOOKUP (REVERSE f) s) (ALOOKUP (REVERSE g) s)’
-            suffices_by (rw [] \\ gs [OPTREL_def]
-                         \\ qpat_x_assum `exp_rel _x _` mp_tac
-                         \\ rw [Once exp_rel_cases] \\ gs [])
-          \\ irule LIST_REL_OPTREL \\ gs []
-          \\ irule LIST_REL_mono
-          \\ first_assum (irule_at Any)
-          \\ simp [ELIM_UNCURRY])
-        \\ drule_then strip_assume_tac ALOOKUP_SOME_REVERSE_EL
-        \\ gvs [EVERY_EL, LIST_REL_EL_EQN]
-        \\ first_x_assum (drule_then strip_assume_tac)
-        \\ gs [ELIM_UNCURRY])
-      \\ reverse (gvs [dest_anyThunk_def, CaseEqs ["option", "exp"]])
-      >- (
-        drule_then strip_assume_tac ALOOKUP_SOME_REVERSE_EL
-        \\ gvs [LIST_REL_EL_EQN]
-        \\ first_x_assum (drule_then strip_assume_tac)
-        \\ gvs [ELIM_UNCURRY])
-      \\ qmatch_asmsub_rename_tac ‘ALOOKUP (REVERSE g) s’
-      \\ ‘OPTREL (λ_x _y. is_delay _x ∧ is_delay _y ∧ exp_rel _x _y)
-                 (ALOOKUP (REVERSE f) s) (ALOOKUP (REVERSE g) s)’
-        by (irule LIST_REL_OPTREL \\ gs []
-            \\ irule LIST_REL_mono
-            \\ first_assum (irule_at Any)
-            \\ simp [ELIM_UNCURRY])
+    \\ Cases_on ‘v1’ \\ Cases_on ‘v2’ \\ gvs [dest_anyThunk_def, dest_Tick_def]
+    >- ((* Recclosure-Recclosure *)
+      rename1 ‘LIST_REL _ xs ys’
+      \\ ‘OPTREL (λ_x _y. is_delay _x ∧ is_delay _y ∧
+                          exp_rel _x _y)
+                 (ALOOKUP (REVERSE xs) s)
+                 (ALOOKUP (REVERSE ys) s)’
+        by (irule LIST_REL_OPTREL
+            \\ gs [LIST_REL_CONJ, ELIM_UNCURRY])
       \\ gs [OPTREL_def]
-      \\ ‘∀m. eval_to (m + j + k) x = eval_to (j + k) x’
-        by (strip_tac
-            \\ irule eval_to_mono \\ simp [])
-      \\ Cases_on ‘_x’ \\ gs []
-      \\ rename1 ‘exp_rel (Delay x1) (Delay x2)’
-      \\ ‘exp_rel (subst_funs f x1) (subst_funs g x2) ∧
-          exp_inv (subst_funs f x1) ∧
-          exp_ok (subst_funs f x1) ∧
-          closed (subst_funs f x1)’
-        by (simp [subst_funs_def, closed_subst]
-            \\ irule_at Any exp_rel_subst
-            \\ irule_at Any exp_inv_subst
-            \\ irule_at Any exp_ok_subst
-            \\ simp [EVERY2_MAP, MAP_MAP_o, combinTheory.o_DEF, LAMBDA_PROD,
-                     GSYM FST_THM]
-            \\ simp [Once thunk_rel_def, EVERY_EL, EL_MAP]
-            \\ irule_at Any LIST_EQ
-            \\ irule_at Any LIST_REL_mono
-            \\ first_assum (irule_at Any)
-            \\ gvs [LIST_REL_EL_EQN, ELIM_UNCURRY, Once exp_rel_cases,
-                    EVERY_EL, EL_MAP, SF SFY_ss] \\ rw []
-            >- (
-              first_x_assum (drule_then strip_assume_tac)
-              \\ Cases_on ‘SND (EL n g)’ \\ gs [])
-            >- (
-              drule_all_then assume_tac exp_ok_eval_to
-              \\ gs [v_ok_def, exp_ok_def, MEM_MAP, EXISTS_PROD, EL_MEM]
-              \\ rw [MEM_EL]
-              \\ first_assum (irule_at Any)
-              \\ Cases_on ‘EL n f’ \\ gs []
-              \\ first_x_assum drule \\ gs [])
-            \\ drule_then strip_assume_tac ALOOKUP_SOME_REVERSE_EL
-            \\ gvs [LIST_REL_EL_EQN, EVERY_EL]
-            \\ rpt (first_x_assum (drule_then strip_assume_tac))
-            \\ gvs [EL_MAP, freevars_def, v_ok_def, EVERY_EL, EL_MAP]
-            \\ last_x_assum (drule_then assume_tac)
-            \\ gs [exp_ok_def])
-      \\ first_x_assum (drule_all_then strip_assume_tac)
-      \\ rename1 ‘_ (eval_to (j1 + k - 1) (subst_funs f x1))’
-      \\ Cases_on ‘eval_to (j1 + k - 1) (subst_funs f x1) =
-                   INL Diverge’ \\ gs []
+      \\ Cases_on ‘_x’ \\ Cases_on ‘_y’ \\ gs []
+      \\ IF_CASES_TAC \\ gs []
+      \\ first_x_assum (qspec_then ‘0’ assume_tac) \\ gs []
+      \\ first_x_assum irule
+      \\ simp [closed_subst, subst_funs_def]
+      \\ irule_at Any exp_rel_subst
+      \\ irule_at Any exp_inv_subst
+      \\ irule_at Any exp_ok_subst
+      \\ simp [EVERY2_MAP, EVERY_MAP, MAP_MAP_o, combinTheory.o_DEF,
+               LAMBDA_PROD, v_ok_def, GSYM FST_THM]
+      \\ irule_at Any LIST_EQ
+      \\ gs [ELIM_UNCURRY, LIST_REL_CONJ]
+      \\ drule_then strip_assume_tac ALOOKUP_SOME_REVERSE_EL
+      \\ gvs [LIST_REL_EL_EQN, EVERY_EL, MEM_EL, PULL_EXISTS, EL_MAP,
+              v_ok_def, EVERY_EL, Once exp_rel_cases, exp_ok_def, exp_inv_def,
+              SF CONJ_ss]
+      \\ rw []
       >- (
-        Cases_on ‘eval_to (j1 + k) x = INL Diverge’ \\ gs []
-        >- (
-          qexists_tac ‘j1’
-          \\ simp [dest_anyThunk_def])
-        \\ ‘eval_to (j1 + k) x = eval_to (j + k) x’
-          by (drule_then (qspec_then ‘j + k’ assume_tac) eval_to_mono
-              \\ ‘eval_to (j + k) x ≠ INL Diverge’ by fs []
-              \\ drule_then (qspec_then ‘j1 + k’ assume_tac) eval_to_mono
-              \\ Cases_on ‘j ≤ j1’ \\ gs [])
-        \\ qexists_tac ‘j1’
-        \\ simp [dest_anyThunk_def])
-      \\ drule_all_then (qspec_then ‘j’ assume_tac) result_rel_mono_left
-      \\ ‘eval_to (j1 + j + k) x = eval_to (j + k) x’
-        by (irule eval_to_mono
-            \\ simp [])
-      \\ qexists_tac ‘j1 + j’
-      \\ gs [dest_anyThunk_def])
-    >- ((* rhs is recclosure *)
-      Cases_on ‘dest_anyThunk (Recclosure g n)’ \\ gs []
-      >- (
-        ‘F’ suffices_by rw []
-        \\ drule_all_then assume_tac exp_rel_exp_ok
-        \\ drule_all_then assume_tac exp_ok_eval_to
-        \\ ‘MEM n (MAP FST g)’ by gs [v_ok_def]
-        \\ Cases_on ‘ALOOKUP (REVERSE g) n’ \\ gs []
-        >- (
-          gs [ALOOKUP_NONE, MAP_REVERSE])
-        \\ ‘∃f. thunk_rel 0 (Recclosure f n) (Recclosure g n)’
-          by (qpat_x_assum ‘thunk_rel _ _ _’ mp_tac
-              \\ rename1 ‘thunk_rel i w _’
-              \\ map_every qid_spec_tac [‘n’, ‘g’, ‘w’, ‘i’]
-              \\ Induct \\ rw []
-              >- (
-                gs [Once thunk_rel_def]
-                \\ rw [Once thunk_rel_def]
-                \\ first_assum (irule_at Any))
-              \\ rw []
-              \\ pop_assum mp_tac
-              \\ rw [Once thunk_rel_def]
-              \\ first_x_assum (drule_then (irule_at Any)))
-        \\ gs [Once thunk_rel_def]
-        \\ drule_then strip_assume_tac ALOOKUP_SOME_REVERSE_EL
-        \\ gvs [LIST_REL_EL_EQN]
-        \\ first_x_assum (drule_then assume_tac)
-        \\ gvs [ELIM_UNCURRY, dest_anyThunk_def, CaseEq "exp"])
-      \\ pairarg_tac \\ gvs []
-      \\ CASE_TAC \\ gs []
-      >- (
-        gs [dest_anyThunk_def, CaseEqs ["option", "exp"]])
-      \\ Cases_on ‘k = 0’ \\ gs []
-      >- (
-        qexists_tac ‘0’
-        \\ Cases_on ‘eval_to 0 x = INL Diverge’ \\ gs []
-        \\ ‘eval_to 0 x = eval_to j x’
-          by (once_rewrite_tac [EQ_SYM_EQ]
-              \\ irule eval_to_mono
-              \\ simp [])
-        \\ gvs [dest_anyThunk_def, CaseEqs ["option", "exp"]])
-      \\ ‘∀m. eval_to (m + j + k) x = eval_to (j + k) x’
-        by (strip_tac
-            \\ irule eval_to_mono
-            \\ simp [])
-      \\ rename1 ‘INR (INR x2, g1)’
-      \\ Cases_on ‘eval_to (k - 1) (subst_funs g1 x2) = INL Diverge’ \\ gs []
-      >- (
-        qexists_tac ‘0’
-        \\ Cases_on ‘eval_to k x = INL Diverge’ \\ gs []
-        \\ ‘eval_to k x = eval_to (j + k) x’
-          by (once_rewrite_tac [EQ_SYM_EQ]
-              \\ irule eval_to_mono
-              \\ simp [])
-        \\ gs [exp_inv_def]
-        \\ last_x_assum assume_tac
-        \\ ntac 5 (last_x_assum kall_tac)
-        \\ gs [v_ok_def, exp_ok_def]
-        \\ map_every (fn tm => qpat_x_assum tm kall_tac) [
-            ‘eval_to k y = _’,
-            ‘eval_to (j + k) x = _’,
-            ‘∀m. eval_to _ _ = _’,
-            ‘eval_to k x = _’ ]
-        \\ qpat_x_assum ‘v_ok w’ mp_tac
-        \\ qpat_x_assum ‘thunk_rel _ _ _’ mp_tac
-        \\ qpat_x_assum ‘thunk_inv _’ mp_tac
-        \\ rename1 ‘thunk_rel m w’
-        \\ qid_spec_tac ‘w’
-        \\ Induct_on ‘m’
-        >- (
-          rw [Once thunk_rel_def]
-          \\ gs [exp_inv_def]
-          \\ ‘OPTREL (λ_x _y. exp_rel _x _y ∧ is_delay _x ∧ is_delay _y)
-                     (ALOOKUP (REVERSE f) n)
-                     (ALOOKUP (REVERSE g) n)’
-            by (irule LIST_REL_OPTREL \\ gs []
-                \\ irule LIST_REL_mono
-                \\ first_assum (irule_at Any)
-                \\ simp [ELIM_UNCURRY])
-          \\ gs [dest_anyThunk_def]
-          \\ simp [Once subst_funs_def, eval_to_def, dest_anyThunk_def]
-          \\ gvs [OPTREL_def, CaseEq "exp"]
-          \\ CASE_TAC \\ gs []
-          \\ IF_CASES_TAC \\ gs []
-          \\ rename1 ‘exp_rel (Delay x1) (Delay x2)’
-          \\ ‘exp_rel (subst_funs f x1) (subst_funs g x2) ∧
-              exp_inv (subst_funs f x1) ∧
-              exp_ok (subst_funs f x1) ∧
-              closed (subst_funs f x1)’
-            by (simp [subst_funs_def, closed_subst, MAP_MAP_o, LAMBDA_PROD,
-                      combinTheory.o_DEF, GSYM FST_THM]
-                \\ irule_at Any exp_rel_subst
-                \\ irule_at Any exp_inv_subst
-                \\ irule_at Any exp_ok_subst
-                \\ simp [MAP_MAP_o, combinTheory.o_DEF, LAMBDA_PROD,
-                         EVERY2_MAP, EVERY_MAP, EVERY_MEM, FORALL_PROD,
-                         Once thunk_rel_def, GSYM FST_THM]
-                \\ irule_at Any LIST_REL_mono
-                \\ first_assum (irule_at Any)
-                \\ simp [ELIM_UNCURRY]
-                \\ irule_at Any LIST_EQ
-                \\ dxrule_then strip_assume_tac ALOOKUP_SOME_REVERSE_EL
-                \\ gvs [LIST_REL_EL_EQN, EL_MAP, ELIM_UNCURRY]
-                \\ first_x_assum (drule_then strip_assume_tac)
-                \\ qpat_x_assum ‘exp_rel (Delay x1) _’ mp_tac
-                \\ rw [Once exp_rel_cases] \\ gs [freevars_def]
-                >- (
-                  gs [v_ok_def, MEM_MAP, EXISTS_PROD, SF SFY_ss])
-                \\ gvs [EVERY_EL, EVERY_MAP, v_ok_def]
-                \\ first_x_assum (drule_then strip_assume_tac)
-                \\ first_x_assum (drule_then strip_assume_tac)
-                \\ gs [exp_ok_def])
-          \\ first_x_assum (drule_all_then strip_assume_tac)
-          \\ rename1 ‘eval_to (j + k - 1) (subst_funs f x1)’
-          \\ Cases_on ‘eval_to (k - 2) (subst_funs f x1) = INL Diverge’ \\ gs []
-          \\ drule_then (qspec_then ‘k - 2 + j + 1’ assume_tac) eval_to_mono
-          \\ gs [])
-        \\ rw [Once thunk_rel_def]
-        \\ fs [thunk_inv_def, exp_inv_def, v_ok_def, exp_ok_def]
-        \\ first_x_assum (drule_all_then assume_tac)
-        \\ simp [dest_anyThunk_def, subst_funs_def]
-        \\ simp [eval_to_def]
-        \\ pop_assum mp_tac
-        \\ gs [eval_to_def, dest_anyThunk_def]
-        \\ gs [subst_funs_def]
-        \\ IF_CASES_TAC \\ gs []
-        \\ Cases_on ‘eval_to (k - 2) (Force (Value u)) = INL Diverge’ \\ gs []
-        \\ drule_then (qspec_then ‘k - 1’ assume_tac) eval_to_mono \\ gs [])
-      \\ Q.REFINE_EXISTS_TAC ‘m + j’
-      \\ gs [exp_inv_def]
-      \\ last_x_assum assume_tac
-      \\ ntac 5 (last_x_assum kall_tac)
-      \\ gs [v_ok_def, exp_ok_def]
-      \\ map_every (fn tm => qpat_x_assum tm kall_tac) [
-          ‘eval_to k y = _’,
-          ‘eval_to (j + k) x = _’,
-          ‘∀m. eval_to _ _ = _’ ]
-      \\ qpat_x_assum ‘v_ok w’ mp_tac
-      \\ qpat_x_assum ‘thunk_rel _ _ _’ mp_tac
-      \\ qpat_x_assum ‘thunk_inv v’ mp_tac
-      \\ rename1 ‘thunk_rel m w’
-      \\ qid_spec_tac ‘w’
-      \\ Induct_on ‘m’
-      >- (
-        rw [Once thunk_rel_def]
-        \\ gs [exp_inv_def]
-        \\ ‘OPTREL (λ_x _y. exp_rel _x _y ∧ is_delay _x ∧ is_delay _y)
-                   (ALOOKUP (REVERSE f) n)
-                   (ALOOKUP (REVERSE g) n)’
-          by (irule LIST_REL_OPTREL \\ gs []
-              \\ irule LIST_REL_mono
-              \\ first_assum (irule_at Any)
-              \\ simp [ELIM_UNCURRY])
-        \\ gs [dest_anyThunk_def]
-        \\ simp [Once subst_funs_def, eval_to_def, dest_anyThunk_def]
-        \\ gvs [OPTREL_def, CaseEq "exp"]
-        \\ CASE_TAC \\ gs []
-        \\ rename1 ‘exp_rel (Delay x1) (Delay x2)’
-        \\ ‘exp_rel (subst_funs f x1) (subst_funs g x2) ∧
-            exp_inv (subst_funs f x1) ∧
-            exp_ok (subst_funs f x1) ∧
-            closed (subst_funs f x1)’
-          by (simp [subst_funs_def, closed_subst, MAP_MAP_o, LAMBDA_PROD,
-                    combinTheory.o_DEF, GSYM FST_THM]
-              \\ irule_at Any exp_rel_subst
-              \\ irule_at Any exp_inv_subst
-              \\ irule_at Any exp_ok_subst
-              \\ simp [MAP_MAP_o, combinTheory.o_DEF, LAMBDA_PROD,
-                       EVERY2_MAP, EVERY_MAP, EVERY_MEM, FORALL_PROD,
-                       Once thunk_rel_def, GSYM FST_THM]
-              \\ irule_at Any LIST_REL_mono
-              \\ first_assum (irule_at Any)
-              \\ simp [ELIM_UNCURRY]
-              \\ irule_at Any LIST_EQ
-              \\ dxrule_then strip_assume_tac ALOOKUP_SOME_REVERSE_EL
-              \\ gvs [LIST_REL_EL_EQN, EL_MAP, ELIM_UNCURRY] \\ rw []
-              >- (
-                gs [v_ok_def, MEM_MAP, EXISTS_PROD, SF SFY_ss])
-              \\ first_x_assum (drule_then strip_assume_tac)
-              \\ qpat_x_assum ‘exp_rel (Delay x1) _’ mp_tac
-              \\ rw [Once exp_rel_cases] \\ gs [freevars_def]
-              \\ gvs [v_ok_def, EVERY_EL, EVERY_MAP, MEM_MAP, EXISTS_PROD,
-                      SF SFY_ss]
-              \\ rw []
-              \\ first_x_assum (drule_then strip_assume_tac) \\ gs [exp_ok_def]
-              \\ first_x_assum (drule_then strip_assume_tac) \\ gs [])
-        \\ first_x_assum (drule_all_then strip_assume_tac)
-        \\ rename1 ‘eval_to (j1 + k - 1) (subst_funs f x1)’
-        \\ qexists_tac ‘j1 + 1’ \\ simp []
-        \\ ‘eval_to (j1 + k - 1) (subst_funs f x1) ≠ INL Diverge’
-          by (strip_tac
-              \\ Cases_on ‘eval_to (k - 1) (subst_funs g x2)’ \\ gs [])
-        \\ dxrule_then (qspec_then ‘j’ assume_tac) result_rel_mono_left
-        \\ gs [])
-      \\ rw [Once thunk_rel_def]
-      \\ fs [thunk_inv_def, exp_inv_def, exp_ok_def, v_ok_def]
-      \\ first_x_assum (drule_all_then (qx_choose_then ‘m1’ assume_tac))
-      \\ simp [dest_anyThunk_def, subst_funs_def]
-      \\ simp [eval_to_def]
-      \\ pop_assum mp_tac
-      \\ rw [eval_to_def, dest_anyThunk_def]
-      \\ gs [subst_funs_def]
-      \\ qexists_tac ‘m1 + 1’ \\ simp [])
-    \\ Cases_on ‘dest_anyThunk v2’ \\ gs []
-    >- (
-      qexists_tac ‘j’
-      \\ gs [dest_anyThunk_def]
-      \\ Cases_on ‘v2’ \\ gs [])
-    \\ Cases_on ‘v2’ \\ gvs [dest_anyThunk_def]
-    \\ Cases_on ‘v1’ \\ gvs [v_rel_Thunk_def]
-    \\ rename1 ‘ss ≠ INR _’
-    \\ Cases_on ‘ss’ \\ gs [])
+        first_assum (irule_at Any) \\ gs [])
+      \\ rpt (first_x_assum (drule_then strip_assume_tac))
+      \\ gs [exp_ok_def, exp_inv_def, freevars_def])
+    >- ((* Thunk-Thunk *)
+      gvs [v_rel_Thunk_def]
+      \\ IF_CASES_TAC \\ gs []
+      \\ first_x_assum (qspec_then ‘0’ assume_tac) \\ gs []
+      \\ first_x_assum irule
+      \\ gs [subst_funs_def, v_ok_def])
+        (* DoTick *)
+    \\ pairarg_tac \\ gvs []
+    \\ simp [arithmeticTheory.ADD1]
+    \\ last_x_assum (qspec_then ‘n + 1’ assume_tac) \\ gs []
+    \\ ‘v = FUNPOW DoTick n w’
+      by (qpat_x_assum ‘dest_Tick v = _’ mp_tac
+          \\ qid_spec_tac ‘n’
+          \\ qid_spec_tac ‘w’
+          \\ qid_spec_tac ‘v’
+          \\ ho_match_mp_tac dest_Tick_ind
+          \\ simp [dest_Tick_def] \\ rw []
+          \\ pairarg_tac \\ gvs []
+          \\ simp [arithmeticTheory.FUNPOW_SUC])
+    \\ cheat (* TODO doesn't work out *))
+  >- ((* MkTick *)
+    rw [Once exp_rel_cases])
   >- ((* Prim *)
     rw [Once exp_rel_cases]
-    \\ gvs [exp_inv_def, eval_to_def]
-    \\ ‘∀n. n < LENGTH xs ⇒ closed (EL n xs)’
-      by gvs [closed_def, freevars_def, LIST_TO_SET_EQ_SING, EVERY_MAP,
-              EVERY_EL]
-    \\ Cases_on ‘op’ \\ gs [exp_ok_def]
+    \\ gvs [exp_ok_def]
+    \\ simp [eval_to_def]
+    \\ Cases_on ‘op’ \\ gs [exp_inv_def, EVERY_EL, EL_MAP, LIST_REL_EL_EQN]
     >- ((* Cons *)
-      gvs [exp_inv_def, result_map_def, MEM_MAP, EL_MAP]
-      \\ simp [eval_to_def, MAP_MAP_o, combinTheory.o_DEF]
+      gvs [result_map_def, MAP_MAP_o, combinTheory.o_DEF, MEM_MAP, eval_to_def,
+           PULL_EXISTS, MEM_EL]
       \\ IF_CASES_TAC \\ gs []
       >- (
-        gvs [EVERY_EL, EVERY_MAP, EVERY2_MAP, PULL_EXISTS, exp_ok_def,
-             exp_inv_def, eval_to_def, MEM_EL, LIST_REL_EL_EQN, PULL_EXISTS]
-        \\ rpt (first_x_assum (drule_all_then strip_assume_tac))
-        \\ gs [eval_to_def])
+        rpt (first_x_assum (drule_then assume_tac))
+        \\ gs [exp_inv_def])
       \\ IF_CASES_TAC \\ gs []
       >- (
-        gvs [EVERY_EL, EVERY_MAP, EVERY2_MAP, PULL_EXISTS, exp_ok_def,
-             exp_inv_def, eval_to_def, MEM_EL, LIST_REL_EL_EQN, PULL_EXISTS]
-        \\ rpt (first_x_assum (drule_all_then strip_assume_tac))
-        \\ gs [eval_to_def])
-      \\ gvs [EVERY_EL, EVERY_MAP, EVERY2_MAP, PULL_EXISTS, exp_ok_def,
-              exp_inv_def, eval_to_def, MEM_EL, LIST_REL_EL_EQN, PULL_EXISTS,
-              v_ok_def, EL_MAP]
+        rpt (first_x_assum (drule_then assume_tac))
+        \\ gs [exp_inv_def])
+      \\ gvs [EVERY2_MAP, EVERY_MAP, v_ok_def, LIST_REL_EL_EQN,
+              EVERY_EL]
       \\ rw []
-      \\ rpt (first_x_assum (drule_all_then strip_assume_tac))
-      \\ Cases_on ‘eval_to k (EL n ys)’ \\ gvs [v_ok_def, v_rel_Thunk_def]
-      >- (
-        irule_at Any thunk_rel_Thunk_Same
-        \\ gs [])
-      \\ irule_at Any thunk_rel_Thunk_Changed \\ gs []
-      \\ first_assum (irule_at Any))
+      \\ rpt (first_x_assum (drule_then assume_tac))
+      \\ Cases_on ‘eval_to k (EL n ys)’ \\ gs [exp_ok_def, exp_inv_def])
     >- ((* IsEq *)
-      drule_then assume_tac LIST_REL_LENGTH
+      IF_CASES_TAC \\ fs []
       \\ IF_CASES_TAC \\ fs []
-      \\ IF_CASES_TAC \\ fs []
-      >- ((* k = 0 *)
-        qexists_tac ‘0’
-        \\ simp [])
       \\ gvs [LENGTH_EQ_NUM_compute, DECIDE “n < 1 ⇔ n = 0”, exp_inv_def]
       \\ rename1 ‘exp_rel x y’
-      \\ first_x_assum (drule_then strip_assume_tac)
-      \\ qexists_tac ‘j’
-      \\ Cases_on ‘eval_to (j + k - 1) x’
-      \\ Cases_on ‘eval_to (k - 1) y’ \\ gs []
+      \\ first_x_assum (drule_all_then assume_tac)
+      \\ Cases_on ‘eval_to (k - 1) x’ \\ Cases_on ‘eval_to (k - 1) y’ \\ gs []
       \\ rename1 ‘v_rel v1 v2’
-      \\ Cases_on ‘dest_Constructor v1’ \\ fs []
-      >- (
-        Cases_on ‘v1’ \\ Cases_on ‘v2’ \\ gs [v_rel_Thunk_def])
-      \\ pairarg_tac \\ gvs []
-      \\ Cases_on ‘v1’ \\ Cases_on ‘v2’ \\ gs [LIST_REL_EL_EQN, v_rel_Thunk_def]
+      \\ Cases_on ‘v1’ \\ Cases_on ‘v2’ \\ gvs []
+      \\ drule_then assume_tac LIST_REL_LENGTH
       \\ IF_CASES_TAC \\ gs [v_ok_def])
     >- ((* Proj *)
       gvs [Once exp_inv_cases])
     >- ((* AtomOp *)
       Cases_on ‘k = 0’ \\ gs []
       >- (
-        qexists_tac ‘0’
-        \\ simp [result_map_def, MEM_MAP]
-        \\ drule_then assume_tac LIST_REL_LENGTH
-        \\ gs [GSYM NOT_NULL_MEM]
-        \\ Cases_on ‘xs’ \\ gs []
-        \\ CASE_TAC \\ gs []
-        \\ CASE_TAC \\ gs [v_ok_def])
-      \\ qmatch_goalsub_abbrev_tac ‘result_map g ys’
-      \\ qabbrev_tac ‘f = λj x. case eval_to (j + k - 1) x of
-                                  INL err => INL err
-                                | INR (Atom l) => INR l
-                                | _ => INL Type_error’
-      \\ simp []
-      \\ qsuff_tac ‘∃j. result_map (f j) xs = result_map g ys’
+        simp [result_map_def, MEM_MAP]
+        \\ gs [GSYM NOT_NULL_MEM, NULL_EQ]
+        \\ Cases_on ‘xs = []’ \\ gs []
+        >- (
+          CASE_TAC \\ gs []
+          \\ CASE_TAC \\ gs [v_ok_def])
+        \\ ‘ys ≠ []’ by (strip_tac \\ gs [])
+        \\ gs [])
+      \\ qmatch_goalsub_abbrev_tac ‘result_map f ys’
+      \\ qsuff_tac ‘result_map f xs = result_map f ys’
       >- (
         rw []
-        \\ qexists_tac ‘j’
-        \\ simp [SF ETA_ss]
-        \\ Cases_on ‘result_map g ys’ \\ gs []
+        \\ Cases_on ‘result_map f ys’ \\ gs []
         \\ CASE_TAC \\ gs []
         \\ CASE_TAC \\ gs [v_ok_def])
-      \\ gvs [LIST_REL_EL_EQN, EVERY_EL, exp_inv_def]
-      \\ Cases_on ‘result_map g ys = INL Diverge’ \\ gs []
+      \\ Cases_on ‘result_map f xs’
       >- (
-        gs [result_map_def, CaseEq "bool", MEM_MAP, MEM_EL, PULL_EXISTS]
-        \\ fs [Once (METIS_PROVE [] “A ⇒ ¬B ⇔ B ⇒ ¬A”)]
-        \\ qexists_tac ‘0’
-        \\ first_assum (irule_at Any)
-        \\ rpt (first_x_assum (drule_all_then strip_assume_tac))
-        \\ unabbrev_all_tac \\ gs []
-        \\ ‘eval_to (k - 1) (EL n ys) = INL Diverge’
-          by gs [CaseEqs ["sum", "v"]]
-        \\ simp [CaseEqs ["sum", "v"]]
-        \\ irule eval_to_Diverge
-        \\ qexists_tac ‘j + k - 1’ \\ simp []
-        \\ Cases_on ‘eval_to (j + k - 1) (EL n xs)’
-        \\ Cases_on ‘eval_to ( k - 1) (EL n ys)’ \\ gs [])
-      \\ ‘∃j.
-            ∀n. n < LENGTH xs ⇒
-              ($= +++ (λv w. v_rel v w ∧ v_inv v ∧ v_ok v))
-                (eval_to (j + k − 1) (EL n xs)) (eval_to (k − 1) (EL n ys))’
-      by (gs [MEM_EL, PULL_EXISTS]
-          \\ rpt (pop_assum mp_tac)
-          \\ qid_spec_tac ‘ys’
-          \\ Induct_on ‘xs’ \\ simp []
-          \\ strip_tac
-          \\ Cases \\ simp []
-          \\ rename1 ‘result_map g (y::ys)’
-          \\ rpt strip_tac
-          \\ last_x_assum (qspec_then ‘ys’ mp_tac)
-          \\ simp [AND_IMP_INTRO]
-          \\ impl_tac
+        Cases_on ‘result_map f ys’
+        >- (
+          gvs [result_map_def, CaseEq "bool", Abbr ‘f’, MEM_MAP, MEM_EL,
+               PULL_EXISTS]
+          \\ fs [Once (DECIDE “A ⇒ ¬B ⇔ B ⇒ ¬A”)]
           >- (
-            rw []
-            \\ ntac 5 (last_x_assum (qspec_then ‘SUC n’ assume_tac)) \\ gs []
-            \\ gs [result_map_def, CaseEq "bool", MEM_MAP]
-            \\ fs [Once (METIS_PROVE [] “A ⇒ ¬B ⇔ B ⇒ ¬A”)])
-          \\ rw []
-          \\ ntac 5 (last_x_assum (qspec_then ‘0’ assume_tac)) \\ gs []
-          \\ first_x_assum (drule_then (qx_choose_then ‘j1’ assume_tac))
-          \\ qexists_tac ‘j1 + j’ \\ gs []
-          \\ Cases \\ simp []
-          >- (
-            drule_then (qspec_then ‘j’ mp_tac) result_rel_mono_left \\ gs []
-            \\ impl_tac \\ rw []
-            \\ strip_tac \\ gs []
-            \\ Cases_on ‘eval_to (k - 1) y’ \\ gvs []
-            \\ gs [Abbr ‘g’, result_map_def, MEM_MAP, CaseEq "bool"])
+            rpt (first_x_assum (drule_then assume_tac))
+            \\ Cases_on ‘eval_to (k - 1) (EL n xs)’
+            \\ gs [CaseEqs ["sum", "v"]])
+          \\ qpat_x_assum ‘n < LENGTH ys’ kall_tac
           \\ rename1 ‘m < LENGTH ys’
-          \\ strip_tac
-          \\ first_x_assum (drule_then assume_tac)
-          \\ drule_then (qspec_then ‘j1’ mp_tac) result_rel_mono_left \\ gs []
-          \\ impl_tac \\ rw []
-          \\ strip_tac \\ gs []
-          \\ Cases_on ‘eval_to (k - 1) (EL m ys)’ \\ gvs []
-          \\ gs [Abbr ‘g’, result_map_def, MEM_MAP, CaseEq "bool",
-                 MEM_EL, PULL_EXISTS])
-      \\ ‘result_map (f j) xs ≠ INL Diverge’
-        by (
-            gs [result_map_def, CaseEq "bool", MEM_MAP]
-            \\ fs [Once (METIS_PROVE [] “A ⇒ ¬B ⇔ B ⇒ ¬A”)] \\ rw []
-            \\ gvs [MEM_EL, PULL_EXISTS]
-            \\ first_x_assum (drule_then assume_tac)
-            \\ strip_tac
-            \\ unabbrev_all_tac \\ gs []
-            \\ rpt (first_x_assum (qspec_then ‘n’ assume_tac))
-            \\ Cases_on ‘eval_to (j + k - 1) (EL n xs)’
-            \\ Cases_on ‘eval_to (k - 1) (EL n ys)’ \\ gvs []
-            \\ gs [CaseEq "v"])
-      \\ qexists_tac ‘j’
-      \\ gs [result_map_def, MAP_MAP_o, combinTheory.o_DEF]
-      \\ IF_CASES_TAC \\ gs []
-      \\ IF_CASES_TAC \\ gs []
+          \\ rpt (first_x_assum (drule_then assume_tac))
+          \\ Cases_on ‘eval_to (k - 1) (EL m ys)’
+          \\ gvs [CaseEqs ["sum", "v"]])
+        \\ gvs [result_map_def, CaseEq "bool", Abbr ‘f’, MEM_MAP, MEM_EL,
+                PULL_EXISTS]
+        \\ fs [Once (DECIDE “A ⇒ ¬B ⇔ B ⇒ ¬A”)]
+        >- (
+          rpt (first_x_assum (drule_then assume_tac))
+          \\ Cases_on ‘eval_to (k - 1) (EL n ys)’
+          \\ gs [CaseEqs ["sum", "v"]])
+        \\ rpt (first_x_assum (drule_then assume_tac))
+        \\ Cases_on ‘eval_to (k - 1) (EL n ys)’
+        \\ gvs [CaseEqs ["sum", "v"], v_rel_Thunk_def])
+      \\ Cases_on ‘result_map f ys’ \\ gs []
       >- (
-        IF_CASES_TAC \\ gs []
-        \\ fs [MEM_MAP, Once (METIS_PROVE [] “A ⇒ ¬B ⇔ B ⇒ ¬A”)]
-        \\ gvs [MEM_EL, PULL_EXISTS]
-        \\ first_assum (irule_at Any)
-        \\ ntac 3 (first_x_assum (drule_then assume_tac))
-        \\ unabbrev_all_tac \\ gs []
-        \\ rpt CASE_TAC \\ gs [CaseEqs ["sum", "v"]])
-      \\ IF_CASES_TAC \\ gs []
-      \\ conj_tac
+        gvs [result_map_def, CaseEq "bool", Abbr ‘f’, MEM_MAP, MEM_EL,
+             PULL_EXISTS]
+        \\ fs [Once (DECIDE “A ⇒ ¬B ⇔ B ⇒ ¬A”)]
+        >- (
+          rpt (first_x_assum (drule_then assume_tac))
+          \\ Cases_on ‘eval_to (k - 1) (EL n xs)’
+          \\ gs [CaseEqs ["sum", "v"]])
+        \\ rpt (first_x_assum (drule_then assume_tac))
+        \\ Cases_on ‘eval_to (k - 1) (EL n xs)’
+        \\ gvs [CaseEqs ["sum", "v"], v_rel_Thunk_def])
+      \\ irule_at Any LIST_EQ
+      \\ gvs [result_map_def, MEM_EL, CaseEq "bool", EL_MAP]
+      \\ fs [Once (DECIDE “A ⇒ ¬B ⇔ B ⇒ ¬A”)] \\ rw []
+      \\ rpt (first_x_assum (drule_then assume_tac))
+      \\ gs [EL_MAP]
+      \\ Cases_on ‘∃err. f (EL x ys) = INL err’ \\ gs []
       >- (
-        fs [MEM_MAP, Once (METIS_PROVE [] “A ⇒ ¬B ⇔ B ⇒ ¬A”)]
-        \\ gvs [MEM_EL, PULL_EXISTS] \\ rw []
-        \\ strip_tac
-        \\ ntac 4 (first_x_assum (drule_then assume_tac))
-        \\ unabbrev_all_tac \\ gs []
-        \\ Cases_on ‘eval_to (j + k - 1) (EL n xs)’
-        \\ Cases_on ‘eval_to (k - 1) (EL n ys)’ \\ gs [CaseEqs ["sum", "v"]]
-        \\ rename1 ‘v_rel v1 _’
-        \\ Cases_on ‘v1’ \\ gs [])
-      \\ irule LIST_EQ
-      \\ gvs [MEM_EL, PULL_EXISTS, EL_MAP]
-      \\ fs [Once (METIS_PROVE [] “A ⇒ ¬B ⇔ B ⇒ ¬A”)]
-      \\ gvs [EL_MAP] \\ rw []
-      \\ ntac 5 (first_x_assum (drule_all_then assume_tac))
-      \\ unabbrev_all_tac \\ gs []
-      \\ rpt CASE_TAC \\ gs []))
+        Cases_on ‘err’ \\ gs [])
+      \\ Cases_on ‘∃err. f (EL x xs) = INL err’ \\ gs []
+      >- (
+        Cases_on ‘err’ \\ gs [])
+      \\ Cases_on ‘f (EL x ys)’ \\ Cases_on ‘f (EL x xs)’ \\ gs []
+      \\ gs [Abbr ‘f’, PULL_EXISTS, CaseEqs ["sum", "v"]]
+      \\ rpt (first_x_assum (drule_then assume_tac)) \\ gs []))
 QED
 
 val _ = export_theory ();
